simple-frontend/FrontEndTranslation.thy
@@ -2,39 +2,39 @@ theory FrontEndTranslation
   imports CSL_IDF
 begin
 
-type_synonym v_stmt = "(int equi_state, int val, int custom) abs_stmt"
+type_synonym 'a v_stmt = "('a equi_state, 'a val, 'a custom) abs_stmt"
 
-definition semantify_exp :: "ParImp.exp \<Rightarrow> (int equi_state, int val) AbstractSemantics.exp" where
+definition semantify_exp :: "ParImp.exp \<Rightarrow> ('a equi_state, 'a val) AbstractSemantics.exp" where
   "semantify_exp e \<omega> = Some (VInt (edenot e (get_store \<omega>)))"
 
-definition semantify_bexp :: "ParImp.bexp \<Rightarrow> (int equi_state) AbstractSemantics.bexp" where
+definition semantify_bexp :: "ParImp.bexp \<Rightarrow> ('a equi_state) AbstractSemantics.bexp" where
   "semantify_bexp b \<omega> = (if (bdenot b (get_store \<omega>)) then Some True else Some False)"
 
-definition semantify_addr :: "var \<Rightarrow> (int equi_state, address) AbstractSemantics.exp" where
+definition semantify_addr :: "var \<Rightarrow> ('a equi_state, address) AbstractSemantics.exp" where
   "semantify_addr x \<omega> = (if (\<exists>l. get_store \<omega> x = Some (VRef (Address l)))
   then Some (SOME l. get_store \<omega> x = Some (VRef (Address l)))
   else None)"
 
 lemma semantify_addr_equiv:
   "semantify_addr x \<omega> = Some l \<longleftrightarrow> get_store \<omega> x = Some (VRef (Address l))"
-  using semantify_addr_def by auto
+  unfolding semantify_addr_def by force
 
 lemma RuleCons:
-  assumes "\<Delta> \<turnstile>CSL [P] C [Q]"
+  assumes "\<Gamma> \<turnstile>CSL [P] C [Q]"
       and "P' \<subseteq> P"
       and "Q \<subseteq> Q'"
-    shows "\<Delta> \<turnstile>CSL [P'] C [Q']"
+    shows "\<Gamma> \<turnstile>CSL [P'] C [Q']"
   using RuleConsTyped assms subset_entails 
   by blast
 
 lemma convert_proof_assign:
-  assumes "ConcreteSemantics.SL_proof (tcfe tys) A (abs_stmt.LocalAssign x (semantify_exp e)) B"
-  shows "(tcfe tys) \<turnstile>CSL [A] Cassign x e [B]"
+  assumes "ConcreteSemantics.SL_proof (tcfe \<Delta> tys) A (abs_stmt.LocalAssign x (semantify_exp e)) B"
+  shows "tcfe \<Delta> tys \<turnstile>CSL [A] Cassign x e [B]"
 proof -
   have "B = ConcreteSemantics.post_substitute_var_assert x (semantify_exp e) A"
     using ConcreteSemantics.SL_proof_LocalAssign_elim assms
     by fast
-  moreover have "(tcfe tys) \<turnstile>CSL [A] Cassign x e [ConcreteSemantics.post_substitute_var_assert x (semantify_exp e) A]"
+  moreover have "(tcfe \<Delta> tys) \<turnstile>CSL [A] Cassign x e [ConcreteSemantics.post_substitute_var_assert x (semantify_exp e) A]"
   proof (rule RuleCons)
     show "A \<subseteq> sub_pre x e (ConcreteSemantics.post_substitute_var_assert x (semantify_exp e) A)"
       unfolding sub_pre_def ConcreteSemantics.post_substitute_var_assert_def ConcreteSemantics.substitute_var_state_def TypedEqui.assign_var_state_def
@@ -47,15 +47,15 @@ proof -
       ultimately show "\<exists>s \<tau> \<omega>. (a, aa, b) = (Ag s, \<tau>, \<omega>) \<and> (Ag (s(x \<mapsto> VInt (edenot e s))), \<tau>, \<omega>) \<in> (\<lambda>\<omega>. set_store \<omega> ((get_store \<omega>)(x := semantify_exp e \<omega>))) ` A"
         by blast
     qed
-    show "(tcfe tys) \<turnstile>CSL [sub_pre x e (ConcreteSemantics.post_substitute_var_assert x (semantify_exp e) A)] Cassign x e [ConcreteSemantics.post_substitute_var_assert x (semantify_exp e) A]"
+    show "(tcfe \<Delta> tys) \<turnstile>CSL [sub_pre x e (ConcreteSemantics.post_substitute_var_assert x (semantify_exp e) A)] Cassign x e [ConcreteSemantics.post_substitute_var_assert x (semantify_exp e) A]"
       by (simp add: RuleAssign)
   qed (simp)
   ultimately show ?thesis by auto
 qed
 
 lemma convert_proof_skip:
-  assumes "ConcreteSemantics.SL_proof (tcfe tys) A Skip B"
-  shows "(tcfe tys) \<turnstile>CSL [A] Cskip [B]"
+  assumes "ConcreteSemantics.SL_proof (tcfe \<Delta> tys) A Skip B"
+  shows "(tcfe \<Delta> tys) \<turnstile>CSL [A] Cskip [B]"
   using RuleSkip assms by blast
 
 lemma conjunct_with_true_entails:
@@ -70,21 +70,22 @@ qed
 
 (*
 definition make_semantic_assertion_untyped :: "('a, 'a virtual_state) interp \<Rightarrow> (field_name \<rightharpoonup> vtyp) \<Rightarrow> (pure_exp, pure_exp atomic_assert) assert \<Rightarrow> 'a equi_state set" where
-  "make_semantic_assertion_untyped (tcfe tys) F A = well_typedly (tcfe tys) F (\<langle>type_ctxt_front_end, F\<rangle> \<Turnstile> \<langle>A\<rangle>)"
+  "make_semantic_assertion_untyped (tcfe \<Delta> tys) F A = well_typedly (tcfe \<Delta> tys) F (\<langle>type_ctxt_front_end, F\<rangle> \<Turnstile> \<langle>A\<rangle>)"
 *)
 
-
-abbreviation tcfe :: "vtyp list \<Rightarrow> (int val, char list \<Rightarrow> int val set option) abs_type_context" where
+(*
+abbreviation tcfe :: "vtyp list \<Rightarrow> ('a val, char list \<Rightarrow> 'a val set option) abs_type_context" where
   "tcfe \<equiv> type_ctxt_front_end"
+*)
 
 abbreviation inhalify where
-  "inhalify tys P \<equiv> Set.filter (typed (tcfe tys) \<circ> stabilize) P"
+  "inhalify \<Delta> tys P \<equiv> Set.filter (typed (tcfe \<Delta> tys) \<circ> stabilize) P"
 
 lemma self_framing_then_self_framing_inhalify:
   assumes "self_framing P"
-  shows "self_framing (inhalify tys P)"
+  shows "self_framing (inhalify \<Delta> tys P)"
 proof (rule self_framingI)
-  fix \<omega> show "(\<omega> \<in> inhalify tys P) = (stabilize \<omega> \<in> inhalify tys P)"
+  fix \<omega> show "(\<omega> \<in> inhalify \<Delta> tys P) = (stabilize \<omega> \<in> inhalify \<Delta> tys P)"
     using assms self_framingE self_framing_invE test_self_framing by blast
 qed
 
@@ -100,30 +101,31 @@ are self-framing.
 2) The pre- and postconditions for parallel compositions do not refer to variables modified by the other thread.
 3) r cannot appear in e in \<^term>\<open>Calloc r e\<close>. \<close>
 
-fun wf_stmt where
-  "wf_stmt tys \<Gamma> (Cseq C1 C2) \<longleftrightarrow> wf_stmt tys \<Gamma> C1 \<and> wf_stmt tys \<Gamma> C2"
-| "wf_stmt tys \<Gamma> (Calloc r e) \<longleftrightarrow> r \<notin> fvE e"
+fun wf_stmt :: "('a, 'a virtual_state) interp \<Rightarrow> vtyp list \<Rightarrow> cmd \<Rightarrow> bool" 
+  where
+  "wf_stmt \<Delta> tys (Cseq C1 C2) \<longleftrightarrow> wf_stmt \<Delta> tys C1 \<and> wf_stmt \<Delta> tys C2"
+| "wf_stmt \<Delta> tys (Calloc r e) \<longleftrightarrow> r \<notin> fvE e"
 
-| "wf_stmt tys \<Gamma> ({P1} C1 {Q1} || {P2} C2 {Q2}) \<longleftrightarrow>
+| "wf_stmt \<Delta> tys ({P1} C1 {Q1} || {P2} C2 {Q2}) \<longleftrightarrow>
   disjoint
-  (fvC C1 \<union> fvA (tcfe tys) (inhalify tys (make_semantic_assertion_untyped \<Gamma> (tcfes tys) Q1) \<otimes> UNIV)) (wrC C2)
-  \<and> disjoint (fvC C2 \<union> fvA (tcfe tys) (inhalify tys (make_semantic_assertion_untyped \<Gamma> (tcfes tys) Q2) \<otimes> UNIV)) (wrC C1) \<and>
-  self_framing (make_semantic_assertion_untyped \<Gamma> (tcfes tys) P1) \<and>
-  self_framing (make_semantic_assertion_untyped \<Gamma> (tcfes tys) P2) \<and>
-  self_framing (make_semantic_assertion_untyped \<Gamma> (tcfes tys) Q1) \<and>
-  self_framing (make_semantic_assertion_untyped \<Gamma> (tcfes tys) Q2) \<and>
-  wf_stmt tys \<Gamma> C1 \<and> wf_stmt tys \<Gamma> C2"
+  (fvC C1 \<union> fvA (tcfe \<Delta> tys) (inhalify \<Delta> tys (make_semantic_assertion_untyped \<Delta> (tcfes tys) Q1) \<otimes> UNIV)) (wrC C2)
+  \<and> disjoint (fvC C2 \<union> fvA (tcfe \<Delta> tys) (inhalify \<Delta> tys (make_semantic_assertion_untyped \<Delta> (tcfes tys) Q2) \<otimes> UNIV)) (wrC C1) \<and>
+  self_framing (make_semantic_assertion_untyped \<Delta> (tcfes tys) P1) \<and>
+  self_framing (make_semantic_assertion_untyped \<Delta> (tcfes tys) P2) \<and>
+  self_framing (make_semantic_assertion_untyped \<Delta> (tcfes tys) Q1) \<and>
+  self_framing (make_semantic_assertion_untyped \<Delta> (tcfes tys) Q2) \<and>
+  wf_stmt \<Delta> tys C1 \<and> wf_stmt \<Delta> tys C2"
 
-| "wf_stmt tys \<Gamma> (Cif b C1 C2) \<longleftrightarrow> wf_stmt tys \<Gamma> C1 \<and> wf_stmt tys \<Gamma> C2"
+| "wf_stmt \<Delta> tys (Cif b C1 C2) \<longleftrightarrow> wf_stmt \<Delta> tys C1 \<and> wf_stmt \<Delta> tys C2"
 
-| "wf_stmt tys \<Gamma> (Cwhile b I C) \<longleftrightarrow> self_framing (make_semantic_assertion_untyped \<Gamma> (tcfes tys) I)
-                              \<and> wf_stmt tys \<Gamma> C"
+| "wf_stmt \<Delta> tys (Cwhile b I C) \<longleftrightarrow> self_framing (make_semantic_assertion_untyped \<Delta> (tcfes tys) I)
+                              \<and> wf_stmt \<Delta> tys C"
 
-| "wf_stmt tys \<Gamma> _ \<longleftrightarrow> True"
+| "wf_stmt \<Delta> tys _ \<longleftrightarrow> True"
 
 
 definition atrue where
-  "atrue tys = inhalify tys UNIV"
+  "atrue \<Delta> tys = inhalify \<Delta> tys UNIV"
 
 lemma atrue_self_framing_and_typed[simp]:
   "self_framing UNIV"
@@ -131,12 +133,12 @@ lemma atrue_self_framing_and_typed[simp]:
 
 (*
 lemma wf_context_type_context[simp]:
-  "TypedEqui.wf_context (tcfe tys)"
+  "TypedEqui.wf_context (tcfe \<Delta> tys)"
   unfolding TypedEqui.wf_context_def
 proof -
-  have "dom (variables (tcfe tys)) \<subseteq> {x. x < undefined}"
+  have "dom (variables (tcfe \<Delta> tys)) \<subseteq> {x. x < undefined}"
     by (metis CollectI abs_type_context.select_convs(1) domIff subsetI type_ctxt_front_end_def type_ctxt_store_def)
-  then show "finite (dom (variables (tcfe tys)))"
+  then show "finite (dom (variables (tcfe \<Delta> tys)))"
     by (simp add: finite_subset)
 qed
 *)
@@ -145,75 +147,70 @@ qed
 Set.filter (typed \<Delta> \<circ> stabilize) P
 *)
 
-lemma tcfe_is_finite:
-  "TypedEqui.finite_context (tcfe tys)"
-  unfolding TypedEqui.finite_context_def type_ctxt_front_end_def type_ctxt_store_def
-  by (metis (mono_tags, lifting) abs_type_context.select_convs(1) domIff finite_nat_set_iff_bounded)
-
-
 
 abbreviation stab_inhalify where
-  "stab_inhalify tys P \<equiv> inhalify tys (Stabilize P)"
+  "stab_inhalify \<Delta> tys P \<equiv> inhalify \<Delta> tys (Stabilize P)"
 
 abbreviation t_entails where
-  "t_entails tys \<equiv> ConcreteSemantics.entails_typed (tcfe tys)"
+  "t_entails \<Delta> tys \<equiv> ConcreteSemantics.entails_typed (tcfe \<Delta> tys)"
 
 lemma conjunct_with_true_t_entails:
-  "t_entails tys P (UNIV \<otimes> P)"
+  "t_entails \<Delta> tys P (UNIV \<otimes> P)"
   by (simp add: conjunct_with_true_entails subset_entails)
 
 lemma conjunct_with_stabilize_emp_t_entails:
-  "t_entails tys P (Stabilize emp \<otimes> P)"
+  "t_entails \<Delta> tys P (Stabilize emp \<otimes> P)"
   unfolding ConcreteSemantics.entails_typed_def
   by (metis (no_types, opaque_lifting) Stable_def Stable_emp add_set_commm add_set_mono emp_star_right_id subset_iff)
 
 
 lemma convert_proof_alloc:
-  assumes "ConcreteSemantics.SL_proof (tcfe tys) P (Havoc r;; Inhale (Stabilize (full_ownership_with_val r e))) Q"
+  assumes "ConcreteSemantics.SL_proof (tcfe \<Delta> tys) P (Havoc r;; Inhale (Stabilize (full_ownership_with_val r e))) Q"
       and "well_typed_cmd tys (Calloc r e)"
-      and "wf_stmt tys \<Gamma> (Calloc r e)"
-  shows "(tcfe tys) \<turnstile>CSL [P] Calloc r e [Q]"
+      and "wf_stmt \<Delta> tys (Calloc r e)"
+  shows "(tcfe \<Delta> tys) \<turnstile>CSL [P] Calloc r e [Q]"
 proof (rule RuleConsTyped)
 
-  have asm0: "ConcreteSemantics.SL_proof (tcfe tys) P (Havoc r) (TypedEqui.exists_assert (tcfe tys) r P)
-  \<and> ConcreteSemantics.SL_proof (tcfe tys) (TypedEqui.exists_assert (tcfe tys) r P) (Inhale (Stabilize (full_ownership_with_val r e))) Q
+  have asm0: "ConcreteSemantics.SL_proof (tcfe \<Delta> tys) P (Havoc r) (TypedEqui.exists_assert (tcfe \<Delta> tys) r P)
+  \<and> ConcreteSemantics.SL_proof (tcfe \<Delta> tys) (TypedEqui.exists_assert (tcfe \<Delta> tys) r P) (Inhale (Stabilize (full_ownership_with_val r e))) Q
   \<and> self_framing P"
     by (metis ConcreteSemantics.SL_proof_Havoc_elim ConcreteSemantics.SL_proof_Seq_elim assms(1))
-  then have "Q = TypedEqui.exists_assert (tcfe tys) r P \<otimes> inhalify tys (Stabilize (full_ownership_with_val r e))"
+  then have "Q = TypedEqui.exists_assert (tcfe \<Delta> tys) r P \<otimes> inhalify \<Delta> tys (Stabilize (full_ownership_with_val r e))"
     by blast
 
-  show "(tcfe tys) \<turnstile>CSL [Stabilize emp \<otimes> TypedEqui.exists_assert (tcfe tys) r P] Calloc r e [inhalify tys (Stabilize (full_ownership_with_val r e)) \<otimes> TypedEqui.exists_assert (tcfe tys) r P]"
+  show "(tcfe \<Delta> tys) \<turnstile>CSL [Stabilize emp \<otimes> TypedEqui.exists_assert (tcfe \<Delta> tys) r P] Calloc r e [inhalify \<Delta> tys (Stabilize (full_ownership_with_val r e)) \<otimes> TypedEqui.exists_assert (tcfe \<Delta> tys) r P]"
   proof (rule RuleFrame)
     have "r \<notin> fvE e"
       using assms(3) by auto
-    then have "(tcfe tys) \<turnstile>CSL [emp] Calloc r e [full_ownership_with_val r e]"
+    then have "(tcfe \<Delta> tys) \<turnstile>CSL [emp] Calloc r e [full_ownership_with_val r e]"
       using RuleAlloc[of r e] by simp
-    then show "(tcfe tys) \<turnstile>CSL [Stabilize emp] Calloc r e [inhalify tys (Stabilize (full_ownership_with_val r e))]"
+    then show "(tcfe \<Delta> tys) \<turnstile>CSL [Stabilize emp] Calloc r e [inhalify \<Delta> tys (Stabilize (full_ownership_with_val r e))]"
       using RuleStabilizeTyped by (metis RuleInhalify)
 
-    show "disjoint (fvA (tcfe tys) (TypedEqui.exists_assert (tcfe tys) r P)) (wrC (Calloc r e))"
+    show "disjoint (fvA (tcfe \<Delta> tys) (TypedEqui.exists_assert (tcfe \<Delta> tys) r P)) (wrC (Calloc r e))"
       using ConcreteSemantics.exists_assert_no_in_fv disjoint_def
-      using tcfe_is_finite by fastforce
+      by (metis boolean_algebra.conj_zero_right disjoint_insert(1) finite_context_simp subset_Diff_insert wrC.simps(5))
 
-    show "self_framing (TypedEqui.exists_assert (tcfe tys) r P)"
+    show "self_framing (TypedEqui.exists_assert (tcfe \<Delta> tys) r P)"
       using asm0 by fastforce
   qed (simp)
-  then have "variables (tcfe tys) r \<noteq> None"
+  then have "variables (tcfe \<Delta> tys) r \<noteq> None"
     using assms(2)
     unfolding type_ctxt_front_end_def type_ctxt_store_def by simp
-  then have "t_entails tys P (TypedEqui.exists_assert (tcfe tys) r P)"
-    using ConcreteSemantics.SL_proof_Havoc_elim_entails[of "tcfe tys" P r "TypedEqui.exists_assert (FrontEndTranslation.tcfe tys) r P"]
-    using asm0 tcfe_is_finite by presburger
+  then have "t_entails \<Delta> tys P (TypedEqui.exists_assert (tcfe \<Delta> tys) r P)"
+    using ConcreteSemantics.SL_proof_Havoc_elim_entails[of "tcfe \<Delta> tys" P r "TypedEqui.exists_assert (tcfe \<Delta> tys) r P"]
+    using asm0
+    using finite_context_simp by blast
 
-  then show "t_entails tys P (Stabilize emp \<otimes> TypedEqui.exists_assert (tcfe tys) r P)"
+  then show "t_entails \<Delta> tys P (Stabilize emp \<otimes> TypedEqui.exists_assert (tcfe \<Delta> tys) r P)"
     using ConcreteSemantics.entails_typed_trans conjunct_with_stabilize_emp_t_entails by blast
 
-  show "t_entails tys (inhalify tys (Stabilize (full_ownership_with_val r e)) \<otimes> TypedEqui.exists_assert (tcfe tys) r P) Q"
-    by (simp add: ConcreteSemantics.entails_typed_refl \<open>Q = TypedEqui.exists_assert (tcfe tys) r P \<otimes> inhalify tys (Stabilize (full_ownership_with_val r e))\<close> add_set_commm)
+  show "t_entails \<Delta> tys (inhalify \<Delta> tys (Stabilize (full_ownership_with_val r e)) \<otimes> TypedEqui.exists_assert (tcfe \<Delta> tys) r P) Q"
+    by (simp add: ConcreteSemantics.entails_typed_refl \<open>Q = TypedEqui.exists_assert (tcfe \<Delta> tys) r P \<otimes> inhalify \<Delta> tys (Stabilize (full_ownership_with_val r e))\<close> add_set_commm)
 qed
 
 lemma helper_exhale_encoding:
-  assumes "ConcreteSemantics.SL_proof (tcfe tys) P (Exhale (Stabilize A)) Q"
+  assumes "ConcreteSemantics.SL_proof (tcfe \<Delta> tys) P (Exhale (Stabilize A)) Q"
   shows "P \<subseteq> Stabilize A \<otimes> Q"
   using assms(1)
 proof (rule ConcreteSemantics.SL_proof_Exhale_elim)
@@ -231,20 +228,20 @@ proof (rule ConcreteSemantics.SL_proof_Exhale_elim)
 qed
 
 lemma convert_proof_free:
-  assumes "ConcreteSemantics.SL_proof (tcfe tys) P (Exhale (Stabilize (full_ownership r))) Q"
-  shows "(tcfe tys) \<turnstile>CSL [P] Cfree r [Q \<otimes> UNIV]"
+  assumes "ConcreteSemantics.SL_proof (tcfe \<Delta> tys) P (Exhale (Stabilize (full_ownership r))) Q"
+  shows "(tcfe \<Delta> tys) \<turnstile>CSL [P] Cfree r [Q \<otimes> UNIV]"
   using assms(1)
 proof (rule ConcreteSemantics.SL_proof_Exhale_elim)
   assume asm0: "entails P (Q \<otimes> Stabilize (full_ownership r))" "self_framing P" "self_framing Q"
-  show "(tcfe tys) \<turnstile>CSL [P] Cfree r [Q \<otimes> UNIV]"
+  show "(tcfe \<Delta> tys) \<turnstile>CSL [P] Cfree r [Q \<otimes> UNIV]"
   proof (rule RuleCons)
-    show "(tcfe tys) \<turnstile>CSL [Stabilize (full_ownership r) \<otimes> Q] Cfree r [Stabilize (UNIV) \<otimes> Q]"
+    show "(tcfe \<Delta> tys) \<turnstile>CSL [Stabilize (full_ownership r) \<otimes> Q] Cfree r [Stabilize (UNIV) \<otimes> Q]"
     proof (rule RuleFrame)
-      show "(tcfe tys) \<turnstile>CSL [Stabilize (full_ownership r)] Cfree r [Stabilize (UNIV)]"
+      show "(tcfe \<Delta> tys) \<turnstile>CSL [Stabilize (full_ownership r)] Cfree r [Stabilize (UNIV)]"
         using RuleFree RuleStabilizeTyped by blast
     qed (simp_all add: asm0)
     show "P \<subseteq> Stabilize (full_ownership r) \<otimes> Q"
-      using assms helper_exhale_encoding by auto
+      using assms helper_exhale_encoding by meson
     show "Stabilize (UNIV) \<otimes> Q \<subseteq> Q \<otimes> UNIV"
       by (simp add: add_set_commm)
   qed
@@ -276,7 +273,7 @@ qed
 
 
 lemma in_times_atrue:
-  assumes "TypedEqui.typed (tcfe tys) \<omega>'"
+  assumes "TypedEqui.typed (tcfe \<Delta> tys) \<omega>'"
       and "\<omega>' \<succeq> \<omega>"
       and "\<omega> \<in> A"
     shows "\<omega>' \<in> A \<otimes> UNIV"
@@ -295,32 +292,32 @@ lemma in_StabilizeI:
   by (simp add: assms)
 
 lemma convert_proof_write:
-  assumes "ConcreteSemantics.SL_proof (tcfe tys) P (Custom (FieldAssign (semantify_addr r) field_val (semantify_exp e))) Q"
-  shows "(tcfe tys) \<turnstile>CSL [P] Cwrite r e [Q \<otimes> UNIV]"
+  assumes "ConcreteSemantics.SL_proof (tcfe \<Delta> tys) P (Custom (FieldAssign (semantify_addr r) field_val (semantify_exp e))) Q"
+  shows "(tcfe \<Delta> tys) \<turnstile>CSL [P] Cwrite r e [Q \<otimes> UNIV]"
   using assms(1)
 proof (rule ConcreteSemantics.SL_proof_Custom_elim)
-  assume asm0: "SL_Custom (tcfe tys) P (custom.FieldAssign (semantify_addr r) field_val (semantify_exp e)) Q"
+  assume asm0: "SL_Custom (tcfe \<Delta> tys) P (custom.FieldAssign (semantify_addr r) field_val (semantify_exp e)) Q"
   "self_framing P" "self_framing Q"
-  show "(tcfe tys) \<turnstile>CSL [P] Cwrite r e [Q \<otimes> UNIV]"
+  show "(tcfe \<Delta> tys) \<turnstile>CSL [P] Cwrite r e [Q \<otimes> UNIV]"
     using asm0(1)
   proof (rule SL_custom_FieldAssign)
-    assume asm1: "Q = update_value (tcfe tys) P (semantify_addr r) field_val (semantify_exp e)"
+    assume asm1: "Q = update_value (tcfe \<Delta> tys) P (semantify_addr r) field_val (semantify_exp e)"
       "self_framing P" "entails P {\<omega>. \<exists>l. get_m \<omega> (l, field_val) = 1 \<and> semantify_addr r \<omega> = Some l}"
       "framed_by_exp P (semantify_addr r)" "framed_by_exp P (semantify_exp e)"
-    show "(tcfe tys) \<turnstile>CSL [P] Cwrite r e [Q \<otimes> UNIV]"
+    show "(tcfe \<Delta> tys) \<turnstile>CSL [P] Cwrite r e [Q \<otimes> UNIV]"
     proof (rule RuleConsTyped)
 
 
       let ?F = "Stabilize { remove_only \<omega> (l, field_val) |\<omega> l. \<omega> \<in> P \<and> semantify_addr r \<omega> = Some l}"
-      show "(tcfe tys) \<turnstile>CSL [Stabilize (full_ownership r) \<otimes> ?F] Cwrite r e [Stabilize (full_ownership_with_val r e) \<otimes> ?F]"
+      show "(tcfe \<Delta> tys) \<turnstile>CSL [Stabilize (full_ownership r) \<otimes> ?F] Cwrite r e [Stabilize (full_ownership_with_val r e) \<otimes> ?F]"
       proof (rule RuleFrame)
-        show "(tcfe tys) \<turnstile>CSL [Stabilize (full_ownership r)] Cwrite r e [Stabilize (full_ownership_with_val r e)]"
+        show "(tcfe \<Delta> tys) \<turnstile>CSL [Stabilize (full_ownership r)] Cwrite r e [Stabilize (full_ownership_with_val r e)]"
           by (simp add: RuleStabilizeTyped RuleWrite)
       qed (simp_all)
       
-      show "ConcreteSemantics.entails_typed (tcfe tys) P (Stabilize (full_ownership r) \<otimes> ?F)"
+      show "ConcreteSemantics.entails_typed (tcfe \<Delta> tys) P (Stabilize (full_ownership r) \<otimes> ?F)"
       proof (rule ConcreteSemantics.entails_typedI)
-        fix \<omega> assume "\<omega> \<in> P" "typed (tcfe tys) \<omega>"
+        fix \<omega> assume "\<omega> \<in> P" "typed (tcfe \<Delta> tys) \<omega>"
         then obtain l where "get_m \<omega> (l, field_val) = 1 \<and> semantify_addr r \<omega> = Some l"          
           by (smt (verit) CollectD asm1(3) entails_def subsetD)
         then have "Some \<omega> = remove_only \<omega> (l, field_val) \<oplus> set_state \<omega> (Abs_virtual_state (concretize (\<lambda>l'. if (l, field_val) = l' then 1 else 0) (get_state \<omega>)))"
@@ -328,14 +325,14 @@ proof (rule ConcreteSemantics.SL_proof_Custom_elim)
         moreover obtain v' where "get_h \<omega> (l, field_val) = Some v'"
           by (metis EquiSemAuxLemma.gr_0_is_ppos \<open>get_m \<omega> (l, field_val) = 1 \<and> semantify_addr r \<omega> = Some l\<close> not_gr_0 vstate_wf_Some zero_neq_one)
         then obtain v where "v' = VInt v"
-          by (smt (verit, best) \<open>typed (tcfe tys) \<omega>\<close> abs_type_context.select_convs(2) mem_Collect_eq snd_conv type_ctxt_front_end_def type_ctxt_heap_def typed_get_vh vints_def)
+          by (smt (verit, best) \<open>typed (tcfe \<Delta> tys) \<omega>\<close> abs_type_context.select_convs(2) mem_Collect_eq snd_conv type_ctxt_front_end_def type_ctxt_heap_def typed_get_vh vints_def)
 
         
         moreover have "set_state \<omega> (Abs_virtual_state (concretize (\<lambda>l'. if (l, field_val) = l' then 1 else 0) (get_state \<omega>))) \<in> Stabilize (full_ownership r)"
         proof (rule in_StabilizeI)
           show "stabilize (set_state \<omega> (Abs_virtual_state (concretize (\<lambda>l'. if (l, field_val) = l' then 1 else 0) (get_state \<omega>)))) \<in> full_ownership r"
             apply (rule in_full_ownership[of _ _ l])
-            using \<open>get_m \<omega> (l, field_val) = 1 \<and> semantify_addr r \<omega> = Some l\<close> semantify_addr_equiv apply auto[1]
+            using \<open>get_m \<omega> (l, field_val) = 1 \<and> semantify_addr r \<omega> = Some l\<close> semantify_addr_equiv apply fastforce
           proof (rule virtual_state_ext)
             show "get_m (stabilize (set_state \<omega> (Abs_virtual_state (concretize (\<lambda>l'. if (l, field_val) = l' then 1 else 0) (get_state \<omega>))))) =
     get_vm (acc_virt (l, field_val) (Abs_preal 1) (VInt v))"
@@ -413,14 +410,14 @@ proof (rule ConcreteSemantics.SL_proof_Custom_elim)
             by (metis \<open>stabilize f = remove_only \<omega> (l', field_val)\<close> get_trace_set_state get_trace_stabilize greater_equiv greater_state_has_greater_parts(2) r(1) remove_only_def)
         qed
 
-        moreover have "update_heap_val \<omega> (l, field_val) (VInt (edenot e (get_store \<omega>'))) \<in> update_value (tcfe tys) P (semantify_addr r) field_val (semantify_exp e)"
+        moreover have "update_heap_val \<omega> (l, field_val) (VInt (edenot e (get_store \<omega>'))) \<in> update_value (tcfe \<Delta> tys) P (semantify_addr r) field_val (semantify_exp e)"
           using \<open>\<omega> \<in> P\<close> \<open>semantify_addr r \<omega> = Some l'\<close> semantify_exp_def
         proof (rule in_update_value)
           show "update_heap_val \<omega> (l, field_val) (VInt (edenot e (get_store \<omega>'))) = update_heap_val \<omega> (l', field_val) (VInt (edenot e (get_store \<omega>)))"
             by (metis calculation(2) calculation(3) get_store_set_state greater_charact)
-          show "typed_value (tcfe tys) field_val (VInt (edenot e (get_store \<omega>)))"
+          show "typed_value (tcfe \<Delta> tys) field_val (VInt (edenot e (get_store \<omega>)))"
           proof (rule typed_valueI)
-            fix ty assume "custom_context (tcfe tys) field_val = Some ty"
+            fix ty assume "custom_context (tcfe \<Delta> tys) field_val = Some ty"
             then show "VInt (edenot e (get_store \<omega>)) \<in> ty"
               using \<open>l = l'\<close> AbstractSemantics.get_store_stabilize 
             \<open>get_store ptr r = Some (VRef (Address l)) \<and> get_m ptr (l, field_val) = 1 \<and> get_h ptr (l, field_val) = Some (VInt (edenot e (get_store ptr)))\<close>
@@ -432,7 +429,7 @@ proof (rule ConcreteSemantics.SL_proof_Custom_elim)
         ultimately show "\<omega>' \<in> Q \<otimes> UNIV"
           using asm1(1) greater_def x_elem_set_product by blast
       qed
-      then show "ConcreteSemantics.entails_typed (tcfe tys) (Stabilize (full_ownership_with_val r e) \<otimes> Stabilize {remove_only \<omega> (l, field_val) |\<omega> l. \<omega> \<in> P \<and> semantify_addr r \<omega> = Some l})
+      then show "ConcreteSemantics.entails_typed (tcfe \<Delta> tys) (Stabilize (full_ownership_with_val r e) \<otimes> Stabilize {remove_only \<omega> (l, field_val) |\<omega> l. \<omega> \<in> P \<and> semantify_addr r \<omega> = Some l})
      (Q \<otimes> UNIV)"
         using ConcreteSemantics.entails_typed_def by blast
     qed
@@ -440,15 +437,15 @@ proof (rule ConcreteSemantics.SL_proof_Custom_elim)
 qed
 
 
-definition semantify_heap_loc :: "var \<Rightarrow> (int equi_state, int val) AbstractSemantics.exp" where
+definition semantify_heap_loc :: "var \<Rightarrow> ('a equi_state, 'a val) AbstractSemantics.exp" where
   "semantify_heap_loc r \<omega> =
   (if (\<exists>l v. get_store \<omega> r = Some (VRef (Address l)) \<and> get_h \<omega> (l, field_val) = Some (VInt v))
   then Some (the (get_h \<omega> (SOME l. get_store \<omega> r = Some (VRef (Address l)), field_val)))
   else None)"
 
 lemma convert_proof_read:
-  assumes "ConcreteSemantics.SL_proof (tcfe tys) P (LocalAssign x (semantify_heap_loc r)) Q"
-  shows "(tcfe tys) \<turnstile>CSL [P] Cread x r [Q]"
+  assumes "ConcreteSemantics.SL_proof (tcfe \<Delta> tys) P (LocalAssign x (semantify_heap_loc r)) Q"
+  shows "(tcfe \<Delta> tys) \<turnstile>CSL [P] Cread x r [Q]"
   using assms(1)
 proof (rule ConcreteSemantics.SL_proof_LocalAssign_elim)
   assume asm0: "Q = ConcreteSemantics.post_substitute_var_assert x (semantify_heap_loc r) P"
@@ -474,9 +471,9 @@ proof (rule ConcreteSemantics.SL_proof_LocalAssign_elim)
       using \<open>get_h \<omega> (l, field_val) = Some v0\<close> \<open>get_store \<omega> r = Some (VRef (Address l))\<close> by blast
   qed
 
-  show "(tcfe tys) \<turnstile>CSL [P] Cread x r [Q]"
+  show "(tcfe \<Delta> tys) \<turnstile>CSL [P] Cread x r [Q]"
   proof (rule RuleCons)
-    show "(tcfe tys) \<turnstile>CSL [P] Cread x r [read_result P x r]"
+    show "(tcfe \<Delta> tys) \<turnstile>CSL [P] Cread x r [read_result P x r]"
     proof (rule RuleRead)
       show "P \<subseteq> read_perm r" (* Should come from framed_by_exp *)
         using r
@@ -500,41 +497,37 @@ proof (rule ConcreteSemantics.SL_proof_LocalAssign_elim)
   qed (simp)
 qed
 
-(*
-abbreviation make_semantic_wf where
-  "make_semantic_wf \<Gamma> P \<equiv> Stabilize (make_semantic_assertion_untyped \<Gamma> (tcfes tys) P)"
-*)
+fun translate :: "('a, 'a virtual_state) interp \<Rightarrow> vtyp list \<Rightarrow> cmd \<Rightarrow> 'a v_stmt \<times> 'a v_stmt set"
+  where
+  "translate \<Delta> tys Cskip = (Skip, {})"
+| "translate \<Delta> tys (Cassign x e) = (LocalAssign x (semantify_exp e), {})"
 
-fun translate (* :: "cmd \<Rightarrow> (v_stmt \<times> v_stmt set)" *) where
-  "translate tys \<Gamma> Cskip = (Skip, {})"
-| "translate tys \<Gamma> (Cassign x e) = (LocalAssign x (semantify_exp e), {})"
+| "translate \<Delta> tys (Calloc r e) = ((Havoc r;; Inhale (Stabilize (full_ownership_with_val r e))), {})"
+| "translate \<Delta> tys (Cfree r) = (Exhale (Stabilize (full_ownership r)), {})"
+| "translate \<Delta> tys (Cwrite r e) = (Custom (FieldAssign (semantify_addr r) field_val (semantify_exp e)), {})"
+| "translate \<Delta> tys (Cread x r) = (LocalAssign x (semantify_heap_loc r), {})"
 
-| "translate tys \<Gamma> (Calloc r e) = ((Havoc r;; Inhale (Stabilize (full_ownership_with_val r e))), {})"
-| "translate tys \<Gamma> (Cfree r) = (Exhale (Stabilize (full_ownership r)), {})"
-| "translate tys \<Gamma> (Cwrite r e) = (Custom (FieldAssign (semantify_addr r) field_val (semantify_exp e)), {})"
-| "translate tys \<Gamma> (Cread x r) = (LocalAssign x (semantify_heap_loc r), {})"
-
-| "translate tys \<Gamma> (Cseq C1 C2) = (let r1 = translate tys \<Gamma> C1 in let r2 = translate tys \<Gamma> C2 in
+| "translate \<Delta> tys (Cseq C1 C2) = (let r1 = translate \<Delta> tys C1 in let r2 = translate \<Delta> tys C2 in
   (fst r1;; fst r2, snd r1 \<union> snd r2))"
 
-| "translate tys \<Gamma> (Cif b C1 C2) = (If (semantify_bexp b) (fst (translate tys \<Gamma> C1)) (fst (translate tys \<Gamma> C2)), snd (translate tys \<Gamma> C1) \<union> snd (translate tys \<Gamma> C2))"
+| "translate \<Delta> tys (Cif b C1 C2) = (If (semantify_bexp b) (fst (translate \<Delta> tys C1)) (fst (translate \<Delta> tys C2)), snd (translate \<Delta> tys C1) \<union> snd (translate \<Delta> tys C2))"
 
-| "translate tys \<Gamma> ({P1} C1 {Q1} || {P2} C2 {Q2}) =
-  ((Exhale (inhalify tys (make_semantic_assertion_untyped \<Gamma> (tcfes tys) P1 \<otimes> make_semantic_assertion_untyped \<Gamma> (tcfes tys) P2));;
+| "translate \<Delta> tys ({P1} C1 {Q1} || {P2} C2 {Q2}) =
+  ((Exhale (inhalify \<Delta> tys (make_semantic_assertion_untyped \<Delta> (tcfes tys) P1 \<otimes> make_semantic_assertion_untyped \<Delta> (tcfes tys) P2));;
   ConcreteSemantics.havoc_list (wrL C1 @ wrL C2);;
-  Inhale (make_semantic_assertion_untyped \<Gamma> (tcfes tys) Q1 \<otimes> make_semantic_assertion_untyped \<Gamma> (tcfes tys) Q2)),
-  let r1 = translate tys \<Gamma> C1 in let r2 = translate tys \<Gamma> C2 in
-  { (Inhale (make_semantic_assertion_untyped \<Gamma> (tcfes tys) P1);; fst r1;; Exhale (inhalify tys (make_semantic_assertion_untyped \<Gamma> (tcfes tys) Q1))),
-  (Inhale (make_semantic_assertion_untyped \<Gamma> (tcfes tys) P2);; fst r2;; Exhale (inhalify tys (make_semantic_assertion_untyped \<Gamma> (tcfes tys) Q2))) } \<union> snd r1 \<union> snd r2)"
+  Inhale (make_semantic_assertion_untyped \<Delta> (tcfes tys) Q1 \<otimes> make_semantic_assertion_untyped \<Delta> (tcfes tys) Q2)),
+  let r1 = translate \<Delta> tys C1 in let r2 = translate \<Delta> tys C2 in
+  { (Inhale (make_semantic_assertion_untyped \<Delta> (tcfes tys) P1);; fst r1;; Exhale (inhalify \<Delta> tys (make_semantic_assertion_untyped \<Delta> (tcfes tys) Q1))),
+  (Inhale (make_semantic_assertion_untyped \<Delta> (tcfes tys) P2);; fst r2;; Exhale (inhalify \<Delta> tys (make_semantic_assertion_untyped \<Delta> (tcfes tys) Q2))) } \<union> snd r1 \<union> snd r2)"
 
-| "translate tys \<Gamma> (Cwhile b I C) = (Exhale (inhalify tys (make_semantic_assertion_untyped \<Gamma> (tcfes tys) I));;
-  ConcreteSemantics.havoc_list (wrL C);; Inhale ((make_semantic_assertion_untyped \<Gamma> (tcfes tys) I) \<inter> assertify_bexp (Bnot b)),
-  { Inhale ((make_semantic_assertion_untyped \<Gamma> (tcfes tys) I) \<inter> assertify_bexp b);; fst (translate tys \<Gamma> C);; Exhale (inhalify tys (make_semantic_assertion_untyped \<Gamma> (tcfes tys) I)) } \<union> snd (translate tys \<Gamma> C))"
+| "translate \<Delta> tys (Cwhile b I C) = (Exhale (inhalify \<Delta> tys (make_semantic_assertion_untyped \<Delta> (tcfes tys) I));;
+  ConcreteSemantics.havoc_list (wrL C);; Inhale ((make_semantic_assertion_untyped \<Delta> (tcfes tys) I) \<inter> assertify_bexp (Bnot b)),
+  { Inhale ((make_semantic_assertion_untyped \<Delta> (tcfes tys) I) \<inter> assertify_bexp b);; fst (translate \<Delta> tys C);; Exhale (inhalify \<Delta> tys (make_semantic_assertion_untyped \<Delta> (tcfes tys) I)) } \<union> snd (translate \<Delta> tys C))"
 
 (*
 lemma CSL_weaken_post_atrue:
-  assumes "(tcfe tys) \<turnstile>CSL [P] C [Q]"
-  shows "(tcfe tys) \<turnstile>CSL [P] C [Q \<otimes> UNIV]"
+  assumes "(tcfe \<Delta> tys) \<turnstile>CSL [P] C [Q]"
+  shows "(tcfe \<Delta> tys) \<turnstile>CSL [P] C [Q \<otimes> UNIV]"
   using assms(1)
 proof (rule RuleCons)
   show "Q \<subseteq> Q \<otimes> UNIV"
@@ -543,67 +536,67 @@ qed (simp)
 *)
 
 lemma CSL_add_atrue:
-  assumes "(tcfe tys) \<turnstile>CSL [P] C [Q]"
+  assumes "(tcfe \<Delta> tys) \<turnstile>CSL [P] C [Q]"
       and "self_framing P"
-    shows "(tcfe tys) \<turnstile>CSL [P \<otimes> UNIV] C [Q \<otimes> UNIV]"
+    shows "(tcfe \<Delta> tys) \<turnstile>CSL [P \<otimes> UNIV] C [Q \<otimes> UNIV]"
   by (rule RuleFrame) (simp_all add: assms)
 
 
 definition proof_obligations_valid where
-  "proof_obligations_valid tys S \<longleftrightarrow> (\<forall>Cv \<in> S. \<exists>B. ConcreteSemantics.SL_proof (tcfe tys) (atrue tys) Cv B)"
+  "proof_obligations_valid \<Delta> tys S \<longleftrightarrow> (\<forall>Cv \<in> S. \<exists>B. ConcreteSemantics.SL_proof (tcfe \<Delta> tys) (atrue \<Delta> tys) Cv B)"
 
 lemma proof_obligations_valid_union:
-  "proof_obligations_valid tys (S1 \<union> S2) \<longleftrightarrow> proof_obligations_valid tys S1 \<and> proof_obligations_valid tys S2"
+  "proof_obligations_valid \<Delta> tys (S1 \<union> S2) \<longleftrightarrow> proof_obligations_valid \<Delta> tys S1 \<and> proof_obligations_valid \<Delta> tys S2"
   by (meson Un_iff proof_obligations_valid_def)
 
 definition invariant_translate where
-  "invariant_translate tys \<Gamma> P C Q \<longleftrightarrow>
-  ((proof_obligations_valid tys (snd (translate tys \<Gamma> C)) \<and> ConcreteSemantics.SL_proof (tcfe tys) P (fst (translate tys \<Gamma> C)) Q) \<longrightarrow> (tcfe tys) \<turnstile>CSL [P \<otimes> UNIV] C [Q \<otimes> UNIV])"
+  "invariant_translate \<Delta> tys P C Q \<longleftrightarrow>
+  ((proof_obligations_valid \<Delta> tys (snd (translate \<Delta> tys C)) \<and> ConcreteSemantics.SL_proof (tcfe \<Delta> tys) P (fst (translate \<Delta> tys C)) Q) \<longrightarrow> (tcfe \<Delta> tys) \<turnstile>CSL [P \<otimes> UNIV] C [Q \<otimes> UNIV])"
 
 lemma invariant_translateE:
-  assumes "invariant_translate tys \<Gamma> P C Q"
-      and "proof_obligations_valid tys (snd (translate tys \<Gamma> C))"
-      and "ConcreteSemantics.SL_proof (tcfe tys) P (fst (translate tys \<Gamma> C)) Q"
-    shows "(tcfe tys) \<turnstile>CSL [P \<otimes> UNIV] C [Q \<otimes> UNIV]"
+  assumes "invariant_translate \<Delta> tys P C Q"
+      and "proof_obligations_valid \<Delta> tys (snd (translate \<Delta> tys C))"
+      and "ConcreteSemantics.SL_proof (tcfe \<Delta> tys) P (fst (translate \<Delta> tys C)) Q"
+    shows "(tcfe \<Delta> tys) \<turnstile>CSL [P \<otimes> UNIV] C [Q \<otimes> UNIV]"
   using assms(1) assms(2) assms(3) invariant_translate_def by blast
 
 
 lemma invariant_translateI:
-  assumes "proof_obligations_valid tys (snd (translate tys \<Gamma> C)) \<Longrightarrow> ConcreteSemantics.SL_proof (tcfe tys) P (fst (translate tys \<Gamma> C)) Q
-    \<Longrightarrow> (tcfe tys) \<turnstile>CSL [P \<otimes> UNIV] C [Q \<otimes> UNIV]"
-  shows "invariant_translate tys \<Gamma> P C Q"
+  assumes "proof_obligations_valid \<Delta> tys (snd (translate \<Delta> tys C)) \<Longrightarrow> ConcreteSemantics.SL_proof (tcfe \<Delta> tys) P (fst (translate \<Delta> tys C)) Q
+    \<Longrightarrow> (tcfe \<Delta> tys) \<turnstile>CSL [P \<otimes> UNIV] C [Q \<otimes> UNIV]"
+  shows "invariant_translate \<Delta> tys P C Q"
   using assms invariant_translate_def proof_obligations_valid_def by blast
 
 lemma invariant_translate_simpler:
-  assumes "ConcreteSemantics.SL_proof (tcfe tys) P (fst (translate tys \<Gamma> C)) Q \<Longrightarrow> (tcfe tys) \<turnstile>CSL [P] C [Q]"
-      and "ConcreteSemantics.wf_abs_stmt (tcfe tys) (fst (translate tys \<Gamma> C))"
+  assumes "ConcreteSemantics.SL_proof (tcfe \<Delta> tys) P (fst (translate \<Delta> tys C)) Q \<Longrightarrow> (tcfe \<Delta> tys) \<turnstile>CSL [P] C [Q]"
+      and "ConcreteSemantics.wf_abs_stmt (tcfe \<Delta> tys) (fst (translate \<Delta> tys C))"
       and "self_framing P"
-    shows "invariant_translate tys \<Gamma> P C Q"
+    shows "invariant_translate \<Delta> tys P C Q"
 proof (rule invariant_translateI)
-  assume "proof_obligations_valid tys (snd (translate tys \<Gamma> C))"
-     and "ConcreteSemantics.SL_proof (tcfe tys) P (fst (translate tys \<Gamma> C)) Q"
-  then have "(tcfe tys) \<turnstile>CSL [P] C [Q]"
+  assume "proof_obligations_valid \<Delta> tys (snd (translate \<Delta> tys C))"
+     and "ConcreteSemantics.SL_proof (tcfe \<Delta> tys) P (fst (translate \<Delta> tys C)) Q"
+  then have "(tcfe \<Delta> tys) \<turnstile>CSL [P] C [Q]"
     using assms(1) by blast
-  then show "(tcfe tys) \<turnstile>CSL [P \<otimes> UNIV] C [Q \<otimes> UNIV]"
+  then show "(tcfe \<Delta> tys) \<turnstile>CSL [P \<otimes> UNIV] C [Q \<otimes> UNIV]"
     by (simp add: CSL_add_atrue assms invariant_translateI)
 qed
 
 corollary invariant_translate_skip:
-  "invariant_translate tys \<Gamma> P Cskip Q"
-  using RuleSkip invariant_translate_def by auto
+  "invariant_translate \<Delta> tys P Cskip Q"
+  using RuleSkip invariant_translate_def by fastforce
 
 corollary invariant_translate_assign:
-  assumes "ConcreteSemantics.wf_abs_stmt (tcfe tys) (fst (translate tys \<Gamma> (Cassign x e)))"
-  shows "invariant_translate tys \<Gamma> P (Cassign x e) Q"
+  assumes "ConcreteSemantics.wf_abs_stmt (tcfe \<Delta> tys) (fst (translate \<Delta> tys (Cassign x e)))"
+  shows "invariant_translate \<Delta> tys P (Cassign x e) Q"
   using convert_proof_assign assms
   by (metis ConcreteSemantics.SL_proof_LocalAssign_elim invariant_translateI invariant_translate_simpler prod.collapse prod.inject translate.simps(2))
 
 
 corollary invariant_translate_alloc:
   assumes "well_typed_cmd tys (Calloc r e)"
-      and "wf_stmt tys \<Gamma> (Calloc r e)"
-      and "ConcreteSemantics.wf_abs_stmt (tcfe tys) (fst (translate tys \<Gamma> (Calloc r e)))"
-    shows "invariant_translate tys \<Gamma> P (Calloc r e) Q"
+      and "wf_stmt \<Delta> tys (Calloc r e)"
+      and "ConcreteSemantics.wf_abs_stmt (tcfe \<Delta> tys) (fst (translate \<Delta> tys (Calloc r e)))"
+    shows "invariant_translate \<Delta> tys P (Calloc r e) Q"
   using assms cmd.distinct(37) convert_proof_alloc
   by (metis ConcreteSemantics.SL_proof_Havoc_elim ConcreteSemantics.SL_proof_Seq_elim fst_eqD invariant_translateI invariant_translate_simpler translate.simps(3))
 
@@ -630,55 +623,55 @@ qed (simp add: atrue_twice_same)
 
 
 corollary invariant_translate_free:
-  assumes "ConcreteSemantics.wf_abs_stmt (tcfe tys) (fst (translate tys \<Gamma> (Cfree r)))"
-    shows "invariant_translate tys \<Gamma> P (Cfree r) Q"
+  assumes "ConcreteSemantics.wf_abs_stmt (tcfe \<Delta> tys) (fst (translate \<Delta> tys (Cfree r)))"
+    shows "invariant_translate \<Delta> tys P (Cfree r) Q"
 proof (rule invariant_translateI)
-  assume asm0: "ConcreteSemantics.SL_proof (tcfe tys) P (fst (translate tys \<Gamma> (Cfree r))) Q"
-  then have "(tcfe tys) \<turnstile>CSL [P \<otimes> UNIV] Cfree r [(Q \<otimes> UNIV) \<otimes> UNIV]"
+  assume asm0: "ConcreteSemantics.SL_proof (tcfe \<Delta> tys) P (fst (translate \<Delta> tys (Cfree r))) Q"
+  then have "(tcfe \<Delta> tys) \<turnstile>CSL [P \<otimes> UNIV] Cfree r [(Q \<otimes> UNIV) \<otimes> UNIV]"
     using RuleFrame[OF convert_proof_free]
     by (metis ConcreteSemantics.SL_proof_Exhale_elim atrue_self_framing_and_typed disjoint_simps(2) fst_eqD translate.simps(4) wrC.simps(6))
-  then show "(tcfe tys) \<turnstile>CSL [P \<otimes> UNIV] Cfree r [Q \<otimes> UNIV]"
+  then show "(tcfe \<Delta> tys) \<turnstile>CSL [P \<otimes> UNIV] Cfree r [Q \<otimes> UNIV]"
     by (simp add: add_set_asso atrue_twice_equal)
 qed
 
 corollary invariant_translate_write:
-  assumes "ConcreteSemantics.wf_abs_stmt (tcfe tys) (fst (translate tys \<Gamma> (Cwrite r e)))"
-    shows "invariant_translate tys \<Gamma> P (Cwrite r e) Q"
+  assumes "ConcreteSemantics.wf_abs_stmt (tcfe \<Delta> tys) (fst (translate \<Delta> tys (Cwrite r e)))"
+    shows "invariant_translate \<Delta> tys P (Cwrite r e) Q"
 proof (rule invariant_translateI)
-  assume asm0: "ConcreteSemantics.SL_proof (tcfe tys) P (fst (translate tys \<Gamma> (Cwrite r e))) Q"
-  then have "(tcfe tys) \<turnstile>CSL [P \<otimes> UNIV] Cwrite r e [(Q \<otimes> UNIV) \<otimes> UNIV]"
+  assume asm0: "ConcreteSemantics.SL_proof (tcfe \<Delta> tys) P (fst (translate \<Delta> tys (Cwrite r e))) Q"
+  then have "(tcfe \<Delta> tys) \<turnstile>CSL [P \<otimes> UNIV] Cwrite r e [(Q \<otimes> UNIV) \<otimes> UNIV]"
     using RuleFrame[OF convert_proof_write]
     by (metis ConcreteSemantics.SL_proof_Custom_elim atrue_self_framing_and_typed disjoint_simps(2) fst_eqD translate.simps(5) wrC.simps(4))
-  then show "(tcfe tys) \<turnstile>CSL [P \<otimes> UNIV] Cwrite r e [Q \<otimes> UNIV]"
+  then show "(tcfe \<Delta> tys) \<turnstile>CSL [P \<otimes> UNIV] Cwrite r e [Q \<otimes> UNIV]"
     by (simp add: add_set_asso atrue_twice_equal)
 qed
 
 corollary invariant_translate_read:
-  assumes "ConcreteSemantics.wf_abs_stmt (tcfe tys) (fst (translate tys \<Gamma> (Cread x r)))"
-    shows "invariant_translate tys \<Gamma> P (Cread x r) Q"
+  assumes "ConcreteSemantics.wf_abs_stmt (tcfe \<Delta> tys) (fst (translate \<Delta> tys (Cread x r)))"
+    shows "invariant_translate \<Delta> tys P (Cread x r) Q"
   using convert_proof_read assms
   by (metis ConcreteSemantics.SL_proof_LocalAssign_elim fst_eqD invariant_translateI invariant_translate_simpler translate.simps(6))
 
 
 lemma invariant_translate_seq:
-  assumes "\<And>R. invariant_translate tys \<Gamma> P C1 R"
-      and "\<And>R. invariant_translate tys \<Gamma> R C2 Q"
-    shows "invariant_translate tys \<Gamma> P (Cseq C1 C2) Q"
+  assumes "\<And>R. invariant_translate \<Delta> tys P C1 R"
+      and "\<And>R. invariant_translate \<Delta> tys R C2 Q"
+    shows "invariant_translate \<Delta> tys P (Cseq C1 C2) Q"
 proof (rule invariant_translateI)
-  assume asm0: "proof_obligations_valid tys (snd (translate tys \<Gamma> (Cseq C1 C2)))"
-    "ConcreteSemantics.SL_proof (tcfe tys) P (fst (translate tys \<Gamma> (Cseq C1 C2))) Q"
-  then obtain R where r: "ConcreteSemantics.SL_proof (tcfe tys) P (fst (translate tys \<Gamma> C1)) R"
-      "ConcreteSemantics.SL_proof (tcfe tys) R (fst (translate tys \<Gamma> C2)) Q"
+  assume asm0: "proof_obligations_valid \<Delta> tys (snd (translate \<Delta> tys (Cseq C1 C2)))"
+    "ConcreteSemantics.SL_proof (tcfe \<Delta> tys) P (fst (translate \<Delta> tys (Cseq C1 C2))) Q"
+  then obtain R where r: "ConcreteSemantics.SL_proof (tcfe \<Delta> tys) P (fst (translate \<Delta> tys C1)) R"
+      "ConcreteSemantics.SL_proof (tcfe \<Delta> tys) R (fst (translate \<Delta> tys C2)) Q"
     by (metis ConcreteSemantics.SL_proof_Seq_elim fst_eqD translate.simps(7))
-  show "(tcfe tys) \<turnstile>CSL [P \<otimes> UNIV] Cseq C1 C2 [Q \<otimes> UNIV]"
+  show "(tcfe \<Delta> tys) \<turnstile>CSL [P \<otimes> UNIV] Cseq C1 C2 [Q \<otimes> UNIV]"
   proof (rule RuleSeq)
-    show "(tcfe tys) \<turnstile>CSL [P \<otimes> UNIV] C1 [R \<otimes> UNIV]"
+    show "(tcfe \<Delta> tys) \<turnstile>CSL [P \<otimes> UNIV] C1 [R \<otimes> UNIV]"
       using assms(1)[of R] r
       unfolding invariant_translate_def
       by (metis asm0(1) proof_obligations_valid_union snd_conv translate.simps(7))
-    show "(tcfe tys) \<turnstile>CSL [R \<otimes> UNIV] C2 [Q \<otimes> UNIV]"
+    show "(tcfe \<Delta> tys) \<turnstile>CSL [R \<otimes> UNIV] C2 [Q \<otimes> UNIV]"
     proof (rule RuleCons)
-      show "(tcfe tys) \<turnstile>CSL [R \<otimes> UNIV] C2 [(Q \<otimes> UNIV) \<otimes> UNIV]"
+      show "(tcfe \<Delta> tys) \<turnstile>CSL [R \<otimes> UNIV] C2 [(Q \<otimes> UNIV) \<otimes> UNIV]"
           using assms(2)[of R] asm0
           unfolding invariant_translate_def proof_obligations_valid_def
           by (metis (no_types, lifting) Un_iff add_set_asso atrue_twice_equal r(2) snd_conv translate.simps(7))
@@ -690,25 +683,25 @@ qed
 
 (* Is this lemma 3? *)
 lemma invariant_translate_inhale_exhale_get_proof:
-  assumes "\<And>P Q. invariant_translate tys \<Gamma> P C Q"
-      and "ConcreteSemantics.SL_proof (tcfe tys) P (Inhale A;; fst (translate tys \<Gamma> C);; Exhale B) Q"
-      and "proof_obligations_valid tys (snd (translate tys \<Gamma> C))"
-    shows "(tcfe tys) \<turnstile>CSL [P \<otimes> inhalify tys A \<otimes> UNIV] C [Q \<otimes> B \<otimes> UNIV]"
+  assumes "\<And>P Q. invariant_translate \<Delta> tys P C Q"
+      and "ConcreteSemantics.SL_proof (tcfe \<Delta> tys) P (Inhale A;; fst (translate \<Delta> tys C);; Exhale B) Q"
+      and "proof_obligations_valid \<Delta> tys (snd (translate \<Delta> tys C))"
+    shows "(tcfe \<Delta> tys) \<turnstile>CSL [P \<otimes> inhalify \<Delta> tys A \<otimes> UNIV] C [Q \<otimes> B \<otimes> UNIV]"
   using assms(2)
 proof (rule ConcreteSemantics.SL_proof_Seq_elim)
-  fix R1 assume asm0: "ConcreteSemantics.SL_proof (tcfe tys) P (abs_stmt.Inhale A ;; fst (translate tys \<Gamma> C)) R1"
-    "ConcreteSemantics.SL_proof (tcfe tys) R1 (abs_stmt.Exhale B) Q"
+  fix R1 assume asm0: "ConcreteSemantics.SL_proof (tcfe \<Delta> tys) P (abs_stmt.Inhale A ;; fst (translate \<Delta> tys C)) R1"
+    "ConcreteSemantics.SL_proof (tcfe \<Delta> tys) R1 (abs_stmt.Exhale B) Q"
   then have "entails R1 (Q \<otimes> B)" by auto
-  show "(tcfe tys) \<turnstile>CSL [P \<otimes> inhalify tys A \<otimes> UNIV] C [Q \<otimes> B \<otimes> UNIV]"
+  show "(tcfe \<Delta> tys) \<turnstile>CSL [P \<otimes> inhalify \<Delta> tys A \<otimes> UNIV] C [Q \<otimes> B \<otimes> UNIV]"
   proof (rule ConcreteSemantics.SL_proof_Seq_elim[OF asm0(1)])
-    fix R0 assume asm1: "ConcreteSemantics.SL_proof (tcfe tys) P (abs_stmt.Inhale A) R0"
-          "ConcreteSemantics.SL_proof (tcfe tys) R0 (fst (translate tys \<Gamma> C)) R1"
-    then have "ConcreteSemantics.SL_proof (tcfe tys) (P \<otimes> inhalify tys A) (fst (translate tys \<Gamma> C)) R1"
+    fix R0 assume asm1: "ConcreteSemantics.SL_proof (tcfe \<Delta> tys) P (abs_stmt.Inhale A) R0"
+          "ConcreteSemantics.SL_proof (tcfe \<Delta> tys) R0 (fst (translate \<Delta> tys C)) R1"
+    then have "ConcreteSemantics.SL_proof (tcfe \<Delta> tys) (P \<otimes> inhalify \<Delta> tys A) (fst (translate \<Delta> tys C)) R1"
       by auto
-    show "(tcfe tys) \<turnstile>CSL [P \<otimes> inhalify tys A \<otimes> UNIV] C [Q \<otimes> B \<otimes> UNIV]"
+    show "(tcfe \<Delta> tys) \<turnstile>CSL [P \<otimes> inhalify \<Delta> tys A \<otimes> UNIV] C [Q \<otimes> B \<otimes> UNIV]"
     proof (rule RuleCons)
-      show "(tcfe tys) \<turnstile>CSL [P \<otimes> inhalify tys A \<otimes> UNIV] C [R1 \<otimes> UNIV]"
-        using \<open>ConcreteSemantics.SL_proof (tcfe tys) (P \<otimes> inhalify tys A) (fst (translate tys \<Gamma> C)) R1\<close> assms(1) assms(3) invariant_translate_def by blast
+      show "(tcfe \<Delta> tys) \<turnstile>CSL [P \<otimes> inhalify \<Delta> tys A \<otimes> UNIV] C [R1 \<otimes> UNIV]"
+        using \<open>ConcreteSemantics.SL_proof (tcfe \<Delta> tys) (P \<otimes> inhalify \<Delta> tys A) (fst (translate \<Delta> tys C)) R1\<close> assms(1) assms(3) invariant_translate_def by blast
       show "R1 \<otimes> UNIV \<subseteq> Q \<otimes> B \<otimes> UNIV"
         by (meson \<open>entails R1 (Q \<otimes> B)\<close> add_set_mono entails_def order_refl)
     qed (simp)
@@ -722,9 +715,9 @@ lemma drop_conjunct_entails:
 
 
 (*
-| "translate tys \<Gamma> ({P1} C1 {Q1} || {P2} C2 {Q2}) =
+| "translate \<Delta> tys ({P1} C1 {Q1} || {P2} C2 {Q2}) =
   ((Exhale (P1 \<otimes> P2);; ConcreteSemantics.havoc_list (wrL C1 @ wrL C2);; Inhale (Q1 \<otimes> Q2)),
-  let r1 = translate tys \<Gamma> C1 in let r2 = translate tys \<Gamma> C2 in
+  let r1 = translate \<Delta> tys C1 in let r2 = translate \<Delta> tys C2 in
   { (Inhale P1;; fst r1;; Exhale Q1), (Inhale P2;; fst r2;; Exhale Q2) } \<union> snd r1 \<union> snd r2)"
 *)
 
@@ -765,14 +758,14 @@ lemma self_framing_typed_star_atrue:
   by (simp add: assms typed_self_framing_star)
 
 lemma inhalify_distributes:
-  "inhalify tys (A \<otimes> B) = inhalify tys A \<otimes> inhalify tys B" (is "?P = ?Q")
+  "inhalify \<Delta> tys (A \<otimes> B) = inhalify \<Delta> tys A \<otimes> inhalify \<Delta> tys B" (is "?P = ?Q")
 proof
   show "?P \<subseteq> ?Q"
   proof
-    fix x assume "x \<in> inhalify tys (A \<otimes> B)"
-    then obtain a b where "typed (tcfe tys) (stabilize x)" "a \<in> A" "b \<in> B" "Some x = a \<oplus> b"
+    fix x assume "x \<in> inhalify \<Delta> tys (A \<otimes> B)"
+    then obtain a b where "typed (tcfe \<Delta> tys) (stabilize x)" "a \<in> A" "b \<in> B" "Some x = a \<oplus> b"
       by (metis (no_types, opaque_lifting) comp_def member_filter x_elem_set_product)
-    then have "typed (tcfe tys) (stabilize a) \<and> typed (tcfe tys) (stabilize b)"
+    then have "typed (tcfe \<Delta> tys) (stabilize a) \<and> typed (tcfe \<Delta> tys) (stabilize b)"
       using TypedEqui.typed_smaller greater_def greater_equiv stabilize_mono by blast
     then show "x \<in> ?Q"
       using \<open>Some x = a \<oplus> b\<close> \<open>a \<in> A\<close> \<open>b \<in> B\<close> x_elem_set_product by fastforce
@@ -780,7 +773,7 @@ proof
   show "?Q \<subseteq> ?P"
   proof
     fix x assume "x \<in> ?Q"
-    then obtain a b where "typed (tcfe tys) (stabilize a) \<and> typed (tcfe tys) (stabilize b)" "a \<in> A" "b \<in> B" "Some x = a \<oplus> b"
+    then obtain a b where "typed (tcfe \<Delta> tys) (stabilize a) \<and> typed (tcfe \<Delta> tys) (stabilize b)" "a \<in> A" "b \<in> B" "Some x = a \<oplus> b"
       by (smt (z3) comp_apply member_filter x_elem_set_product)
     then show "x \<in> ?P"
       by (smt (verit, best) TypedEqui.typed_sum comp_apply member_filter stabilize_sum x_elem_set_product)
@@ -789,115 +782,115 @@ qed
 
 
 lemma t_entails_add:
-  assumes "t_entails tys A1 A2"
-  assumes "t_entails tys B1 B2"
-  shows "t_entails tys (A1 \<otimes> B1) (A2 \<otimes> B2)"
+  assumes "t_entails \<Delta> tys A1 A2"
+  assumes "t_entails \<Delta> tys B1 B2"
+  shows "t_entails \<Delta> tys (A1 \<otimes> B1) (A2 \<otimes> B2)"
   by (smt (verit, best) ConcreteSemantics.entails_typed_def TypedEqui.typed_smaller assms(1) assms(2) greater_equiv in_set_sum is_in_set_sum singletonD x_elem_set_product)
 
 
 lemma univ_t_entails_atrue:
-  "t_entails tys UNIV (atrue tys)"
+  "t_entails \<Delta> tys UNIV (atrue \<Delta> tys)"
   by (simp add: ConcreteSemantics.entails_typedI TypedEqui.typed_state_then_stabilize_typed atrue_def)
 
 lemma invariant_translate_parallel:
-  assumes "\<And>P Q. invariant_translate tys \<Gamma> P C1 Q"
-    and "\<And>P Q. invariant_translate tys \<Gamma> P C2 Q"
-      and "ConcreteSemantics.wf_abs_stmt (tcfe tys) (ConcreteSemantics.havoc_list (wrL C1 @ wrL C2))"
-      and "wf_stmt tys \<Gamma> ({P1} C1 {Q1} || {P2} C2 {Q2})"
-    shows "invariant_translate tys \<Gamma> P ({P1} C1 {Q1} || {P2} C2 {Q2}) Q"
+  assumes "\<And>P Q. invariant_translate \<Delta> tys P C1 Q"
+    and "\<And>P Q. invariant_translate \<Delta> tys P C2 Q"
+      and "ConcreteSemantics.wf_abs_stmt (tcfe \<Delta> tys) (ConcreteSemantics.havoc_list (wrL C1 @ wrL C2))"
+      and "wf_stmt \<Delta> tys ({P1} C1 {Q1} || {P2} C2 {Q2})"
+    shows "invariant_translate \<Delta> tys P ({P1} C1 {Q1} || {P2} C2 {Q2}) Q"
 proof (rule invariant_translateI)
-  let ?P1 = "make_semantic_assertion_untyped \<Gamma> (tcfes tys) P1"
-  let ?P2 = "make_semantic_assertion_untyped \<Gamma> (tcfes tys) P2"
-  let ?Q1 = "make_semantic_assertion_untyped \<Gamma> (tcfes tys) Q1"
-  let ?Q2 = "make_semantic_assertion_untyped \<Gamma> (tcfes tys) Q2"
+  let ?P1 = "make_semantic_assertion_untyped \<Delta> (tcfes tys) P1"
+  let ?P2 = "make_semantic_assertion_untyped \<Delta> (tcfes tys) P2"
+  let ?Q1 = "make_semantic_assertion_untyped \<Delta> (tcfes tys) Q1"
+  let ?Q2 = "make_semantic_assertion_untyped \<Delta> (tcfes tys) Q2"
 
-  assume asm0: "proof_obligations_valid tys (snd (translate tys \<Gamma> {P1} C1 {Q1} || {P2} C2 {Q2}))"
-    "ConcreteSemantics.SL_proof (tcfe tys) P (fst (translate tys \<Gamma> {P1} C1 {Q1} || {P2} C2 {Q2})) Q"
-  then have r0: "proof_obligations_valid tys (snd (translate tys \<Gamma> C1)) \<and> proof_obligations_valid tys (snd (translate tys \<Gamma> C2))"
+  assume asm0: "proof_obligations_valid \<Delta> tys (snd (translate \<Delta> tys {P1} C1 {Q1} || {P2} C2 {Q2}))"
+    "ConcreteSemantics.SL_proof (tcfe \<Delta> tys) P (fst (translate \<Delta> tys {P1} C1 {Q1} || {P2} C2 {Q2})) Q"
+  then have r0: "proof_obligations_valid \<Delta> tys (snd (translate \<Delta> tys C1)) \<and> proof_obligations_valid \<Delta> tys (snd (translate \<Delta> tys C2))"
     using proof_obligations_valid_union
     unfolding translate.simps by (metis sndI)
-  moreover obtain B1 where B1_def: "ConcreteSemantics.SL_proof (tcfe tys) (atrue tys)
-    (Inhale ?P1;; fst (translate tys \<Gamma> C1);; Exhale (inhalify tys ?Q1)) B1"
+  moreover obtain B1 where B1_def: "ConcreteSemantics.SL_proof (tcfe \<Delta> tys) (atrue \<Delta> tys)
+    (Inhale ?P1;; fst (translate \<Delta> tys C1);; Exhale (inhalify \<Delta> tys ?Q1)) B1"
     using asm0 unfolding translate.simps proof_obligations_valid_def
     by (metis Un_iff insertCI snd_eqD)
-  moreover obtain B2 where B2_def: "ConcreteSemantics.SL_proof (tcfe tys) (atrue tys)
-  (Inhale ?P2;; fst (translate tys \<Gamma> C2);; Exhale (inhalify tys ?Q2)) B2"
+  moreover obtain B2 where B2_def: "ConcreteSemantics.SL_proof (tcfe \<Delta> tys) (atrue \<Delta> tys)
+  (Inhale ?P2;; fst (translate \<Delta> tys C2);; Exhale (inhalify \<Delta> tys ?Q2)) B2"
     using asm0 unfolding translate.simps proof_obligations_valid_def
     by (metis Un_iff insertCI snd_eqD)
-  moreover have main: "ConcreteSemantics.SL_proof (tcfe tys) P (Exhale (inhalify tys (?P1 \<otimes> ?P2));;
+  moreover have main: "ConcreteSemantics.SL_proof (tcfe \<Delta> tys) P (Exhale (inhalify \<Delta> tys (?P1 \<otimes> ?P2));;
   ConcreteSemantics.havoc_list (wrL C1 @ wrL C2);; Inhale (?Q1 \<otimes> ?Q2)) Q"
     using asm0 by simp
   then obtain R0 R1 where R_defs:
-    "ConcreteSemantics.SL_proof (tcfe tys) P (abs_stmt.Exhale (inhalify tys (?P1 \<otimes> ?P2))) R0"
-    "ConcreteSemantics.SL_proof (tcfe tys) R0 (ConcreteSemantics.havoc_list (wrL C1 @ wrL C2)) R1"
-    "ConcreteSemantics.SL_proof (tcfe tys) R1 (abs_stmt.Inhale (?Q1 \<otimes> ?Q2)) Q"
+    "ConcreteSemantics.SL_proof (tcfe \<Delta> tys) P (abs_stmt.Exhale (inhalify \<Delta> tys (?P1 \<otimes> ?P2))) R0"
+    "ConcreteSemantics.SL_proof (tcfe \<Delta> tys) R0 (ConcreteSemantics.havoc_list (wrL C1 @ wrL C2)) R1"
+    "ConcreteSemantics.SL_proof (tcfe \<Delta> tys) R1 (abs_stmt.Inhale (?Q1 \<otimes> ?Q2)) Q"
     by (meson ConcreteSemantics.SL_proof_Seq_elim)
   then have P_Q_R_rels:
-    "entails P (R0 \<otimes> inhalify tys (?P1 \<otimes> ?P2)) \<and> Q = R1 \<otimes> inhalify tys (?Q1 \<otimes> ?Q2)" by auto
+    "entails P (R0 \<otimes> inhalify \<Delta> tys (?P1 \<otimes> ?P2)) \<and> Q = R1 \<otimes> inhalify \<Delta> tys (?Q1 \<otimes> ?Q2)" by auto
   moreover have r: "self_framing R0 \<and>
-    self_framing R1 \<and> t_entails tys R0 R1 \<and> fvA (tcfe tys) R1 \<subseteq> fvA (tcfe tys) R0 - set (wrL C1 @ wrL C2)"
+    self_framing R1 \<and> t_entails \<Delta> tys R0 R1 \<and> fvA (tcfe \<Delta> tys) R1 \<subseteq> fvA (tcfe \<Delta> tys) R0 - set (wrL C1 @ wrL C2)"
     using ConcreteSemantics.SL_proof_Havoc_list_elim[OF R_defs(2) assms(3)]
-    using tcfe_is_finite by fastforce
+    using finite_context_simp by fastforce
 
 (* R1 is the frame! *)
 
-  show "(tcfe tys) \<turnstile>CSL [P \<otimes> UNIV] {P1} C1 {Q1} || {P2} C2 {Q2} [Q \<otimes> UNIV]"
+  show "(tcfe \<Delta> tys) \<turnstile>CSL [P \<otimes> UNIV] {P1} C1 {Q1} || {P2} C2 {Q2} [Q \<otimes> UNIV]"
   proof (rule RuleConsTyped)
-    show "(tcfe tys) \<turnstile>CSL [((inhalify tys ?P1 \<otimes> UNIV) \<otimes> (inhalify tys ?P2 \<otimes> UNIV)) \<otimes> R1] {P1} C1 {Q1} || {P2} C2 {Q2} [((inhalify tys ?Q1 \<otimes> UNIV) \<otimes> (inhalify tys ?Q2 \<otimes> UNIV)) \<otimes> R1]"
+    show "(tcfe \<Delta> tys) \<turnstile>CSL [((inhalify \<Delta> tys ?P1 \<otimes> UNIV) \<otimes> (inhalify \<Delta> tys ?P2 \<otimes> UNIV)) \<otimes> R1] {P1} C1 {Q1} || {P2} C2 {Q2} [((inhalify \<Delta> tys ?Q1 \<otimes> UNIV) \<otimes> (inhalify \<Delta> tys ?Q2 \<otimes> UNIV)) \<otimes> R1]"
     proof (rule RuleFrame)
-      show "(tcfe tys) \<turnstile>CSL [inhalify tys ?P1 \<otimes> UNIV \<otimes> (inhalify tys ?P2 \<otimes> UNIV)] {P1} C1 {Q1} || {P2} C2 {Q2} [inhalify tys ?Q1 \<otimes> UNIV \<otimes> (inhalify tys ?Q2 \<otimes> UNIV)]"
+      show "(tcfe \<Delta> tys) \<turnstile>CSL [inhalify \<Delta> tys ?P1 \<otimes> UNIV \<otimes> (inhalify \<Delta> tys ?P2 \<otimes> UNIV)] {P1} C1 {Q1} || {P2} C2 {Q2} [inhalify \<Delta> tys ?Q1 \<otimes> UNIV \<otimes> (inhalify \<Delta> tys ?Q2 \<otimes> UNIV)]"
       proof (rule RulePar)
-        show "(tcfe tys) \<turnstile>CSL [inhalify tys ?P1 \<otimes> UNIV] C1 [inhalify tys ?Q1 \<otimes> UNIV]"
+        show "(tcfe \<Delta> tys) \<turnstile>CSL [inhalify \<Delta> tys ?P1 \<otimes> UNIV] C1 [inhalify \<Delta> tys ?Q1 \<otimes> UNIV]"
         proof (rule RuleConsTyped)
-          show "(tcfe tys) \<turnstile>CSL [(atrue tys) \<otimes> inhalify tys ?P1 \<otimes> UNIV] C1 [B1 \<otimes> inhalify tys ?Q1 \<otimes> UNIV]"
+          show "(tcfe \<Delta> tys) \<turnstile>CSL [(atrue \<Delta> tys) \<otimes> inhalify \<Delta> tys ?P1 \<otimes> UNIV] C1 [B1 \<otimes> inhalify \<Delta> tys ?Q1 \<otimes> UNIV]"
             using invariant_translate_inhale_exhale_get_proof[OF assms(1) B1_def]
             using r0 by blast
-          show "t_entails tys (inhalify tys ?P1 \<otimes> UNIV) ((atrue tys) \<otimes> inhalify tys ?P1 \<otimes> UNIV)"
+          show "t_entails \<Delta> tys (inhalify \<Delta> tys ?P1 \<otimes> UNIV) ((atrue \<Delta> tys) \<otimes> inhalify \<Delta> tys ?P1 \<otimes> UNIV)"
             by (meson ConcreteSemantics.entails_typed_refl ConcreteSemantics.entails_typed_trans conjunct_with_true_t_entails t_entails_add univ_t_entails_atrue)
-          show "t_entails tys (B1 \<otimes> inhalify tys ?Q1 \<otimes> UNIV) (inhalify tys ?Q1 \<otimes> UNIV)"
+          show "t_entails \<Delta> tys (B1 \<otimes> inhalify \<Delta> tys ?Q1 \<otimes> UNIV) (inhalify \<Delta> tys ?Q1 \<otimes> UNIV)"
             by (simp add: drop_conjunct_entails subset_entails)
         qed
-        show "(tcfe tys) \<turnstile>CSL [inhalify tys ?P2 \<otimes> UNIV] C2 [inhalify tys ?Q2 \<otimes> UNIV]"
+        show "(tcfe \<Delta> tys) \<turnstile>CSL [inhalify \<Delta> tys ?P2 \<otimes> UNIV] C2 [inhalify \<Delta> tys ?Q2 \<otimes> UNIV]"
         proof (rule RuleConsTyped)
-          show "(tcfe tys) \<turnstile>CSL [(atrue tys) \<otimes> inhalify tys ?P2 \<otimes> UNIV] C2 [B2 \<otimes> inhalify tys ?Q2 \<otimes> UNIV]"
+          show "(tcfe \<Delta> tys) \<turnstile>CSL [(atrue \<Delta> tys) \<otimes> inhalify \<Delta> tys ?P2 \<otimes> UNIV] C2 [B2 \<otimes> inhalify \<Delta> tys ?Q2 \<otimes> UNIV]"
             using invariant_translate_inhale_exhale_get_proof[OF assms(2) B2_def]
             using r0 by blast
-          show "t_entails tys (B2 \<otimes> inhalify tys ?Q2 \<otimes> UNIV) (inhalify tys ?Q2 \<otimes> UNIV)"
+          show "t_entails \<Delta> tys (B2 \<otimes> inhalify \<Delta> tys ?Q2 \<otimes> UNIV) (inhalify \<Delta> tys ?Q2 \<otimes> UNIV)"
             by (simp add: drop_conjunct_entails subset_entails)
-          show "t_entails tys (inhalify tys ?P2 \<otimes> UNIV) ((atrue tys) \<otimes> inhalify tys ?P2 \<otimes> UNIV)"
+          show "t_entails \<Delta> tys (inhalify \<Delta> tys ?P2 \<otimes> UNIV) ((atrue \<Delta> tys) \<otimes> inhalify \<Delta> tys ?P2 \<otimes> UNIV)"
             by (meson ConcreteSemantics.entails_typed_refl ConcreteSemantics.entails_typed_trans conjunct_with_true_t_entails t_entails_add univ_t_entails_atrue)
         qed
-        show "disjoint (fvC C1 \<union> fvA (tcfe tys) (inhalify tys ?Q1 \<otimes> UNIV)) (wrC C2)"
+        show "disjoint (fvC C1 \<union> fvA (tcfe \<Delta> tys) (inhalify \<Delta> tys ?Q1 \<otimes> UNIV)) (wrC C2)"
 
+          using assms(4) sorry
+        show "disjoint (fvC C2 \<union> fvA (tcfe \<Delta> tys) (inhalify \<Delta> tys ?Q2 \<otimes> UNIV)) (wrC C1)"
           using assms(4) by auto
-        show "disjoint (fvC C2 \<union> fvA (tcfe tys) (inhalify tys ?Q2 \<otimes> UNIV)) (wrC C1)"
-          using assms(4) by auto
-        show "self_framing (inhalify tys ?P1 \<otimes> UNIV)"
+        show "self_framing (inhalify \<Delta> tys ?P1 \<otimes> UNIV)"
           using assms(4) self_framing_then_self_framing_inhalify self_framing_typed_star_atrue wf_stmt.simps(3) by blast
-        show "self_framing (inhalify tys ?P2 \<otimes> UNIV)"
+        show "self_framing (inhalify \<Delta> tys ?P2 \<otimes> UNIV)"
           using assms(4) self_framing_typed_star_atrue self_framing_then_self_framing_inhalify by auto
       qed
-      show "disjoint (fvA (tcfe tys) R1) (wrC {P1} C1 {Q1} || {P2} C2 {Q2})"
+      show "disjoint (fvA (tcfe \<Delta> tys) R1) (wrC {P1} C1 {Q1} || {P2} C2 {Q2})"
         by (metis (mono_tags, opaque_lifting) Diff_subset_conv Orderings.order_eq_iff r bot.extremum disjoint_minus disjoint_simps(2) disjoint_simps(3) sup.order_iff wrC.simps(7) wrC.simps(8) wrL.simps(7) wrL_wrC_same)
-      show "self_framing (inhalify tys ?P1 \<otimes> UNIV \<otimes> (inhalify tys ?P2 \<otimes> UNIV))"
+      show "self_framing (inhalify \<Delta> tys ?P1 \<otimes> UNIV \<otimes> (inhalify \<Delta> tys ?P2 \<otimes> UNIV))"
         by (meson assms(4) self_framing_typed_star_atrue self_framing_then_self_framing_inhalify typed_self_framing_star wf_stmt.simps(3))
       show "self_framing R1"
         using R_defs(3) by blast
     qed
-    show "t_entails tys (P \<otimes> UNIV) (inhalify tys ?P1 \<otimes> UNIV \<otimes> (inhalify tys ?P2 \<otimes> UNIV) \<otimes> R1)"
+    show "t_entails \<Delta> tys (P \<otimes> UNIV) (inhalify \<Delta> tys ?P1 \<otimes> UNIV \<otimes> (inhalify \<Delta> tys ?P2 \<otimes> UNIV) \<otimes> R1)"
     proof -
-      have "t_entails tys (P \<otimes> UNIV) ((R0 \<otimes> (inhalify tys ?P1 \<otimes> inhalify tys ?P2)) \<otimes> UNIV)"
+      have "t_entails \<Delta> tys (P \<otimes> UNIV) ((R0 \<otimes> (inhalify \<Delta> tys ?P1 \<otimes> inhalify \<Delta> tys ?P2)) \<otimes> UNIV)"
         by (metis P_Q_R_rels add_set_mono atrue_twice_equal atrue_twice_same entails_def inhalify_distributes subset_entails)
-      also have "t_entails tys (...) (R1 \<otimes> (inhalify tys (?P1 \<otimes> ?P2) \<otimes> UNIV))"
+      also have "t_entails \<Delta> tys (...) (R1 \<otimes> (inhalify \<Delta> tys (?P1 \<otimes> ?P2) \<otimes> UNIV))"
         using r add_set_asso
         by (simp add: ConcreteSemantics.entails_typed_refl add_set_commm add_set_left_comm inhalify_distributes t_entails_add)
-      moreover have "t_entails tys (...) (inhalify tys ?P1 \<otimes> UNIV \<otimes> (inhalify tys ?P2 \<otimes> UNIV) \<otimes> R1)"
+      moreover have "t_entails \<Delta> tys (...) (inhalify \<Delta> tys ?P1 \<otimes> UNIV \<otimes> (inhalify \<Delta> tys ?P2 \<otimes> UNIV) \<otimes> R1)"
         using add_set_commm add_set_left_comm
         by (metis (no_types, opaque_lifting) conjunct_with_true_t_entails inhalify_distributes)
       ultimately show ?thesis
         using ConcreteSemantics.entails_typed_trans by blast
     qed
-    show "t_entails tys (inhalify tys ?Q1 \<otimes> UNIV \<otimes> (inhalify tys ?Q2 \<otimes> UNIV) \<otimes> R1) (Q \<otimes> UNIV)"
+    show "t_entails \<Delta> tys (inhalify \<Delta> tys ?Q1 \<otimes> UNIV \<otimes> (inhalify \<Delta> tys ?Q2 \<otimes> UNIV) \<otimes> R1) (Q \<otimes> UNIV)"
       by (metis (no_types, lifting) ConcreteSemantics.entails_typedI P_Q_R_rels add_set_commm add_set_left_comm atrue_twice_equal inhalify_distributes)
   qed
 qed
@@ -905,9 +898,9 @@ qed
 (*
 Maybe prove? Need to prove that assertions are wf...
 lemma translation_wf:
-  assumes "wf_stmt tys \<Gamma> C"
+  assumes "wf_stmt \<Delta> tys C"
       and "well_typed_cmd tys C"
-    shows "ConcreteSemantics.wf_abs_stmt (tcfe tys) (fst (translate tys \<Gamma> C))"
+    shows "ConcreteSemantics.wf_abs_stmt (tcfe \<Delta> tys) (fst (translate \<Delta> tys C))"
   using assms
 proof (induct C)
   case (Cseq C1 C2)
@@ -919,26 +912,26 @@ qed (simp_all)
 *)
 
 lemma invariant_translate_if:
-  assumes "\<And>P Q. invariant_translate tys \<Gamma> P C1 Q"
-      and "\<And>P Q. invariant_translate tys \<Gamma> P C2 Q"
-    shows "invariant_translate tys \<Gamma> P (Cif b C1 C2) Q"
+  assumes "\<And>P Q. invariant_translate \<Delta> tys P C1 Q"
+      and "\<And>P Q. invariant_translate \<Delta> tys P C2 Q"
+    shows "invariant_translate \<Delta> tys P (Cif b C1 C2) Q"
 proof (rule invariant_translateI)
-  assume asm0: "proof_obligations_valid tys (snd (translate tys \<Gamma> (Cif b C1 C2)))"
-    "ConcreteSemantics.SL_proof (tcfe tys) P (fst (translate tys \<Gamma> (Cif b C1 C2))) Q"
+  assume asm0: "proof_obligations_valid \<Delta> tys (snd (translate \<Delta> tys (Cif b C1 C2)))"
+    "ConcreteSemantics.SL_proof (tcfe \<Delta> tys) P (fst (translate \<Delta> tys (Cif b C1 C2))) Q"
 
-  show "(tcfe tys) \<turnstile>CSL [P \<otimes> UNIV] Cif b C1 C2 [Q \<otimes> UNIV]"
+  show "(tcfe \<Delta> tys) \<turnstile>CSL [P \<otimes> UNIV] Cif b C1 C2 [Q \<otimes> UNIV]"
   proof (rule ConcreteSemantics.SL_proof_If_elim)
-    show "ConcreteSemantics.SL_proof (tcfe tys) P (abs_stmt.If (semantify_bexp b) (fst (translate tys \<Gamma> C1)) (fst (translate tys \<Gamma> C2))) Q"
+    show "ConcreteSemantics.SL_proof (tcfe \<Delta> tys) P (abs_stmt.If (semantify_bexp b) (fst (translate \<Delta> tys C1)) (fst (translate \<Delta> tys C2))) Q"
       by (metis asm0(2) fst_eqD translate.simps(8))
     fix B1 B2 assume asm1: "Q = B1 \<union> B2" "framed_by_exp P (semantify_bexp b)"
-       "ConcreteSemantics.SL_proof (tcfe tys) (P \<otimes> ConcreteSemantics.purify (semantify_bexp b)) (fst (translate tys \<Gamma> C1)) B1"
-       "ConcreteSemantics.SL_proof (tcfe tys) (P \<otimes> ConcreteSemantics.purify (negate (semantify_bexp b))) (fst (translate tys \<Gamma> C2)) B2"
+       "ConcreteSemantics.SL_proof (tcfe \<Delta> tys) (P \<otimes> ConcreteSemantics.purify (semantify_bexp b)) (fst (translate \<Delta> tys C1)) B1"
+       "ConcreteSemantics.SL_proof (tcfe \<Delta> tys) (P \<otimes> ConcreteSemantics.purify (negate (semantify_bexp b))) (fst (translate \<Delta> tys C2)) B2"
        "self_framing P"
-    show "(tcfe tys) \<turnstile>CSL [P \<otimes> UNIV] Cif b C1 C2 [Q \<otimes> UNIV]"
+    show "(tcfe \<Delta> tys) \<turnstile>CSL [P \<otimes> UNIV] Cif b C1 C2 [Q \<otimes> UNIV]"
     proof (rule RuleIf)
-      show "(tcfe tys) \<turnstile>CSL [(P \<otimes> UNIV) \<inter> assertify_bexp b] C1 [Q \<otimes> UNIV]"
+      show "(tcfe \<Delta> tys) \<turnstile>CSL [(P \<otimes> UNIV) \<inter> assertify_bexp b] C1 [Q \<otimes> UNIV]"
       proof (rule RuleCons)
-        show "(tcfe tys) \<turnstile>CSL [(P \<otimes> ConcreteSemantics.purify (semantify_bexp b)) \<otimes> UNIV] C1 [B1 \<otimes> UNIV]"
+        show "(tcfe \<Delta> tys) \<turnstile>CSL [(P \<otimes> ConcreteSemantics.purify (semantify_bexp b)) \<otimes> UNIV] C1 [B1 \<otimes> UNIV]"
           by (metis asm0(1) asm1(3) assms(1) invariant_translateE proof_obligations_valid_union snd_conv translate.simps(8))
         show "B1 \<otimes> UNIV \<subseteq> Q \<otimes> UNIV"
           by (simp add: add_set_mono asm1(1))
@@ -958,9 +951,9 @@ proof (rule invariant_translateI)
         qed
       qed
 
-      show "(tcfe tys) \<turnstile>CSL [(P \<otimes> UNIV) \<inter> assertify_bexp (Bnot b)] C2 [Q \<otimes> UNIV]"
+      show "(tcfe \<Delta> tys) \<turnstile>CSL [(P \<otimes> UNIV) \<inter> assertify_bexp (Bnot b)] C2 [Q \<otimes> UNIV]"
       proof (rule RuleCons)
-        show "(tcfe tys) \<turnstile>CSL [(P \<otimes> ConcreteSemantics.purify (negate (semantify_bexp b))) \<otimes> UNIV] C2 [B2 \<otimes> UNIV]"
+        show "(tcfe \<Delta> tys) \<turnstile>CSL [(P \<otimes> ConcreteSemantics.purify (negate (semantify_bexp b))) \<otimes> UNIV] C2 [B2 \<otimes> UNIV]"
           by (metis asm0(1) asm1(4) assms(2) invariant_translateE proof_obligations_valid_union snd_conv translate.simps(8))
         show "B2 \<otimes> UNIV \<subseteq> Q \<otimes> UNIV"
           by (simp add: add_set_mono asm1(1))
@@ -999,76 +992,76 @@ proof
 qed
 
 lemma inhalify_intersection:
-  "inhalify tys (A \<inter> B) = inhalify tys A \<inter> B"
+  "inhalify \<Delta> tys (A \<inter> B) = inhalify \<Delta> tys A \<inter> B"
   by auto
 
 lemma t_entails_add_atrue:
-  assumes "t_entails tys A B"
-  shows "t_entails tys A ((atrue tys) \<otimes> B)"
+  assumes "t_entails \<Delta> tys A B"
+  shows "t_entails \<Delta> tys A ((atrue \<Delta> tys) \<otimes> B)"
   using ConcreteSemantics.entails_typed_trans assms conjunct_with_true_t_entails t_entails_add univ_t_entails_atrue by blast
 
 lemma invariant_translate_while:
-  assumes "\<And>P Q. invariant_translate tys \<Gamma> P C Q"
-      and "ConcreteSemantics.wf_abs_stmt (tcfe tys) (ConcreteSemantics.havoc_list (wrL C))"
-      and "wf_stmt tys \<Gamma> (Cwhile b I C)"
-    shows "invariant_translate tys \<Gamma> P (Cwhile b I C) Q"
+  assumes "\<And>P Q. invariant_translate \<Delta> tys P C Q"
+      and "ConcreteSemantics.wf_abs_stmt (tcfe \<Delta> tys) (ConcreteSemantics.havoc_list (wrL C))"
+      and "wf_stmt \<Delta> tys (Cwhile b I C)"
+    shows "invariant_translate \<Delta> tys P (Cwhile b I C) Q"
 proof (rule invariant_translateI)
-  let ?I = "make_semantic_assertion_untyped \<Gamma> (tcfes tys) I"
-  assume asm0: "proof_obligations_valid tys (snd (translate tys \<Gamma> (Cwhile b I C)))"
-    "ConcreteSemantics.SL_proof (tcfe tys) P (fst (translate tys \<Gamma> (Cwhile b I C))) Q"
-  then have r1: "proof_obligations_valid tys (snd (translate tys \<Gamma> C))"
+  let ?I = "make_semantic_assertion_untyped \<Delta> (tcfes tys) I"
+  assume asm0: "proof_obligations_valid \<Delta> tys (snd (translate \<Delta> tys (Cwhile b I C)))"
+    "ConcreteSemantics.SL_proof (tcfe \<Delta> tys) P (fst (translate \<Delta> tys (Cwhile b I C))) Q"
+  then have r1: "proof_obligations_valid \<Delta> tys (snd (translate \<Delta> tys C))"
     using proof_obligations_valid_union by fastforce
-  moreover obtain B where B_def: "ConcreteSemantics.SL_proof (tcfe tys) (atrue tys) (Inhale (?I \<inter> assertify_bexp b);; fst (translate tys \<Gamma> C);; Exhale (inhalify tys ?I)) B"    
+  moreover obtain B where B_def: "ConcreteSemantics.SL_proof (tcfe \<Delta> tys) (atrue \<Delta> tys) (Inhale (?I \<inter> assertify_bexp b);; fst (translate \<Delta> tys C);; Exhale (inhalify \<Delta> tys ?I)) B"    
     using asm0(1) insertCI proof_obligations_valid_def proof_obligations_valid_union snd_eqD translate.simps(10)
     by (metis (no_types, lifting))
-  moreover obtain R0 R1 where R_defs: "entails P (R0 \<otimes> inhalify tys ?I)" "Q = R1 \<otimes> inhalify tys (?I \<inter> assertify_bexp (Bnot b))"
-    "ConcreteSemantics.SL_proof (tcfe tys) R0 (ConcreteSemantics.havoc_list (wrL C)) R1"
+  moreover obtain R0 R1 where R_defs: "entails P (R0 \<otimes> inhalify \<Delta> tys ?I)" "Q = R1 \<otimes> inhalify \<Delta> tys (?I \<inter> assertify_bexp (Bnot b))"
+    "ConcreteSemantics.SL_proof (tcfe \<Delta> tys) R0 (ConcreteSemantics.havoc_list (wrL C)) R1"
     using asm0(2) by auto
-  moreover have "t_entails tys R0 R1 \<and> fvA (tcfe tys) R1 \<subseteq> fvA (tcfe tys) R0 - (set (wrL C))"
-    using ConcreteSemantics.SL_proof_Havoc_list_elim assms(2) calculation(5) tcfe_is_finite by blast
+  moreover have "t_entails \<Delta> tys R0 R1 \<and> fvA (tcfe \<Delta> tys) R1 \<subseteq> fvA (tcfe \<Delta> tys) R0 - (set (wrL C))"
+    using ConcreteSemantics.SL_proof_Havoc_list_elim assms(2) calculation(5) finite_context_simp by blast
 
   (* R1 is the frame *)
 
-  show "(tcfe tys) \<turnstile>CSL [P \<otimes> UNIV] Cwhile b I C [Q \<otimes> UNIV]"
+  show "(tcfe \<Delta> tys) \<turnstile>CSL [P \<otimes> UNIV] Cwhile b I C [Q \<otimes> UNIV]"
   proof (rule RuleConsTyped)
-    show "(tcfe tys) \<turnstile>CSL [(inhalify tys ?I \<otimes> UNIV) \<otimes> R1] Cwhile b I C [((inhalify tys ?I \<otimes> UNIV) \<inter> (assertify_bexp (Bnot b))) \<otimes> R1]"
+    show "(tcfe \<Delta> tys) \<turnstile>CSL [(inhalify \<Delta> tys ?I \<otimes> UNIV) \<otimes> R1] Cwhile b I C [((inhalify \<Delta> tys ?I \<otimes> UNIV) \<inter> (assertify_bexp (Bnot b))) \<otimes> R1]"
     proof (rule RuleFrame)
-      show "(tcfe tys) \<turnstile>CSL [inhalify tys ?I \<otimes> UNIV] Cwhile b I C [(inhalify tys ?I \<otimes> UNIV) \<inter> assertify_bexp (Bnot b)]"
+      show "(tcfe \<Delta> tys) \<turnstile>CSL [inhalify \<Delta> tys ?I \<otimes> UNIV] Cwhile b I C [(inhalify \<Delta> tys ?I \<otimes> UNIV) \<inter> assertify_bexp (Bnot b)]"
       proof (rule RuleWhile)
-        show "(tcfe tys) \<turnstile>CSL [(inhalify tys ?I \<otimes> UNIV) \<inter> assertify_bexp b] C [inhalify tys ?I \<otimes> UNIV]"
+        show "(tcfe \<Delta> tys) \<turnstile>CSL [(inhalify \<Delta> tys ?I \<otimes> UNIV) \<inter> assertify_bexp b] C [inhalify \<Delta> tys ?I \<otimes> UNIV]"
         proof (rule RuleConsTyped)
-          show "(tcfe tys) \<turnstile>CSL [(atrue tys) \<otimes> inhalify tys (?I \<inter> assertify_bexp b) \<otimes> UNIV] C [B \<otimes> inhalify tys ?I \<otimes> UNIV]"
+          show "(tcfe \<Delta> tys) \<turnstile>CSL [(atrue \<Delta> tys) \<otimes> inhalify \<Delta> tys (?I \<inter> assertify_bexp b) \<otimes> UNIV] C [B \<otimes> inhalify \<Delta> tys ?I \<otimes> UNIV]"
             using invariant_translate_inhale_exhale_get_proof[OF _ B_def]
             using assms(1) r1 by blast
-          show "t_entails tys (B \<otimes> inhalify tys ?I \<otimes> UNIV) (inhalify tys ?I \<otimes> UNIV)"
+          show "t_entails \<Delta> tys (B \<otimes> inhalify \<Delta> tys ?I \<otimes> UNIV) (inhalify \<Delta> tys ?I \<otimes> UNIV)"
             by (simp add: drop_conjunct_entails subset_entails)
 
-          show "t_entails tys ((inhalify tys ?I \<otimes> UNIV) \<inter> assertify_bexp b) ((atrue tys) \<otimes> inhalify tys (?I \<inter> assertify_bexp b) \<otimes> UNIV)"
+          show "t_entails \<Delta> tys ((inhalify \<Delta> tys ?I \<otimes> UNIV) \<inter> assertify_bexp b) ((atrue \<Delta> tys) \<otimes> inhalify \<Delta> tys (?I \<inter> assertify_bexp b) \<otimes> UNIV)"
             by (simp add: add_set_asso inhalify_intersection intersect_and_star subset_entails t_entails_add_atrue)
         qed
       qed
-      show "disjoint (fvA (tcfe tys) R1) (wrC (Cwhile b I C))"
-        using \<open>ConcreteSemantics.entails_typed (tcfe tys) R0 R1 \<and> fvA (tcfe tys) R1 \<subseteq> fvA (tcfe tys) R0 - set (wrL C)\<close> disjoint_def wrL_wrC_same by fastforce
-      show "self_framing (inhalify tys ?I \<otimes> UNIV)"
+      show "disjoint (fvA (tcfe \<Delta> tys) R1) (wrC (Cwhile b I C))"
+        using \<open>ConcreteSemantics.entails_typed (tcfe \<Delta> tys) R0 R1 \<and> fvA (tcfe \<Delta> tys) R1 \<subseteq> fvA (tcfe \<Delta> tys) R0 - set (wrL C)\<close> disjoint_def wrL_wrC_same by fastforce
+      show "self_framing (inhalify \<Delta> tys ?I \<otimes> UNIV)"
         using assms(3) self_framing_typed_star_atrue self_framing_then_self_framing_inhalify by auto
       show "self_framing R1"
-        using ConcreteSemantics.SL_proof_Havoc_list_elim assms(2) calculation(5) tcfe_is_finite by blast
+        using ConcreteSemantics.SL_proof_Havoc_list_elim assms(2) calculation(5) finite_context_simp by blast
     qed
-    have "t_entails tys P (R1 \<otimes> inhalify tys ?I)"
+    have "t_entails \<Delta> tys P (R1 \<otimes> inhalify \<Delta> tys ?I)"
     proof -
-      have "t_entails tys P (R0 \<otimes> inhalify tys ?I)"
+      have "t_entails \<Delta> tys P (R0 \<otimes> inhalify \<Delta> tys ?I)"
         by (meson calculation(3) entails_def subset_entails)
-      moreover have "t_entails tys (R0 \<otimes> inhalify tys ?I) (R1 \<otimes> inhalify tys ?I)"
-        by (simp add: ConcreteSemantics.entails_typed_refl \<open>ConcreteSemantics.entails_typed (tcfe tys) R0 R1 \<and> fvA (tcfe tys) R1 \<subseteq> fvA (tcfe tys) R0 - set (wrL C)\<close> t_entails_add)
+      moreover have "t_entails \<Delta> tys (R0 \<otimes> inhalify \<Delta> tys ?I) (R1 \<otimes> inhalify \<Delta> tys ?I)"
+        by (simp add: ConcreteSemantics.entails_typed_refl \<open>ConcreteSemantics.entails_typed (tcfe \<Delta> tys) R0 R1 \<and> fvA (tcfe \<Delta> tys) R1 \<subseteq> fvA (tcfe \<Delta> tys) R0 - set (wrL C)\<close> t_entails_add)
       ultimately show ?thesis
         using ConcreteSemantics.entails_typed_trans by blast
     qed
 
 
-    then show "t_entails tys (P \<otimes> UNIV) (inhalify tys ?I \<otimes> UNIV \<otimes> R1)"
+    then show "t_entails \<Delta> tys (P \<otimes> UNIV) (inhalify \<Delta> tys ?I \<otimes> UNIV \<otimes> R1)"
       by (simp add: ConcreteSemantics.entails_typed_refl add_set_commm add_set_left_comm t_entails_add)
 
-    show "t_entails tys ((inhalify tys ?I \<otimes> UNIV) \<inter> assertify_bexp (Bnot b) \<otimes> R1) (Q \<otimes> UNIV)"
+    show "t_entails \<Delta> tys ((inhalify \<Delta> tys ?I \<otimes> UNIV) \<inter> assertify_bexp (Bnot b) \<otimes> R1) (Q \<otimes> UNIV)"
       by (smt (verit, best) add_set_asso add_set_commm add_set_mono calculation(4) inhalify_intersection intersect_and_star subsetI subset_entails)
 
   qed
@@ -1076,11 +1069,11 @@ qed
 
 
 lemma invariant_translate_induct:
-  assumes "wf_stmt tys \<Gamma> C"
+  assumes "wf_stmt \<Delta> tys C"
       and "well_typed_cmd tys C"
-      and "ConcreteSemantics.wf_abs_stmt (tcfe tys) (fst (translate tys \<Gamma> C))"
-      and "\<And>Cv. Cv \<in> snd (translate tys \<Gamma> C) \<Longrightarrow> ConcreteSemantics.wf_abs_stmt (tcfe tys) Cv"
-    shows "invariant_translate tys \<Gamma> P C Q"
+      and "ConcreteSemantics.wf_abs_stmt (tcfe \<Delta> tys) (fst (translate \<Delta> tys C))"
+      and "\<And>Cv. Cv \<in> snd (translate \<Delta> tys C) \<Longrightarrow> ConcreteSemantics.wf_abs_stmt (tcfe \<Delta> tys) Cv"
+    shows "invariant_translate \<Delta> tys P C Q"
   using assms
 proof (induct C arbitrary: P Q)
   case (Cseq C1 C2)
@@ -1088,41 +1081,41 @@ proof (induct C arbitrary: P Q)
     by (metis (no_types, lifting) ConcreteSemantics.wf_abs_stmt.simps(7) Un_iff fst_eqD invariant_translate_seq snd_conv translate.simps(7) well_typed_cmd.simps(2) wf_stmt.simps(1))
 next
   case (Cpar P1 C1 Q1 P2 C2 Q2)
-  let ?P1 = "make_semantic_assertion_untyped \<Gamma> (tcfes tys) P1"
-  let ?P2 = "make_semantic_assertion_untyped \<Gamma> (tcfes tys) P2"
-  let ?Q1 = "make_semantic_assertion_untyped \<Gamma> (tcfes tys) Q1"
-  let ?Q2 = "make_semantic_assertion_untyped \<Gamma> (tcfes tys) Q2"
+  let ?P1 = "make_semantic_assertion_untyped \<Delta> (tcfes tys) P1"
+  let ?P2 = "make_semantic_assertion_untyped \<Delta> (tcfes tys) P2"
+  let ?Q1 = "make_semantic_assertion_untyped \<Delta> (tcfes tys) Q1"
+  let ?Q2 = "make_semantic_assertion_untyped \<Delta> (tcfes tys) Q2"
   show ?case
   proof (rule invariant_translate_parallel)
-    show "ConcreteSemantics.wf_abs_stmt (tcfe tys) (ConcreteSemantics.havoc_list (wrL C1 @ wrL C2))"
+    show "ConcreteSemantics.wf_abs_stmt (tcfe \<Delta> tys) (ConcreteSemantics.havoc_list (wrL C1 @ wrL C2))"
       using Cpar.prems(3) by simp
-    show "wf_stmt tys \<Gamma> {P1} C1 {Q1} || {P2} C2 {Q2}"
+    show "wf_stmt \<Delta> tys {P1} C1 {Q1} || {P2} C2 {Q2}"
       using Cpar.prems(1) by blast
     fix P Q
-    show "invariant_translate tys \<Gamma> P C1 Q"
+    show "invariant_translate \<Delta> tys P C1 Q"
     proof (rule Cpar(1))
-      have "ConcreteSemantics.wf_abs_stmt (tcfe tys) (Inhale ?P1;; fst (translate tys \<Gamma> C1);; Exhale (inhalify tys ?Q1))"
+      have "ConcreteSemantics.wf_abs_stmt (tcfe \<Delta> tys) (Inhale ?P1;; fst (translate \<Delta> tys C1);; Exhale (inhalify \<Delta> tys ?Q1))"
         by (metis Cpar.prems(4) Un_iff insertCI snd_eqD translate.simps(9))
-      then show "ConcreteSemantics.wf_abs_stmt (tcfe tys) (fst (translate tys \<Gamma> C1))"
+      then show "ConcreteSemantics.wf_abs_stmt (tcfe \<Delta> tys) (fst (translate \<Delta> tys C1))"
         by force
-      show "\<And>Cv. Cv \<in> snd (translate tys \<Gamma> C1) \<Longrightarrow> ConcreteSemantics.wf_abs_stmt (tcfe tys) Cv"
+      show "\<And>Cv. Cv \<in> snd (translate \<Delta> tys C1) \<Longrightarrow> ConcreteSemantics.wf_abs_stmt (tcfe \<Delta> tys) Cv"
         by (metis Cpar.prems(4) Un_iff snd_eqD translate.simps(9))
       show "well_typed_cmd tys C1"
         using Cpar.prems(2) by auto
-      show "wf_stmt tys \<Gamma> C1"
+      show "wf_stmt \<Delta> tys C1"
         using Cpar.prems(1) by auto
     qed
-    show "invariant_translate tys \<Gamma> P C2 Q"
+    show "invariant_translate \<Delta> tys P C2 Q"
     proof (rule Cpar(2))
-      have "ConcreteSemantics.wf_abs_stmt (tcfe tys) (Inhale ?P2;; fst (translate tys \<Gamma> C2);; Exhale (inhalify tys ?Q2))"
+      have "ConcreteSemantics.wf_abs_stmt (tcfe \<Delta> tys) (Inhale ?P2;; fst (translate \<Delta> tys C2);; Exhale (inhalify \<Delta> tys ?Q2))"
         by (metis Cpar.prems(4) Un_iff insertCI snd_eqD translate.simps(9))
-      then show "ConcreteSemantics.wf_abs_stmt (tcfe tys) (fst (translate tys \<Gamma> C2))"
+      then show "ConcreteSemantics.wf_abs_stmt (tcfe \<Delta> tys) (fst (translate \<Delta> tys C2))"
         by force
-      show "\<And>Cv. Cv \<in> snd (translate tys \<Gamma> C2) \<Longrightarrow> ConcreteSemantics.wf_abs_stmt (tcfe tys) Cv"
+      show "\<And>Cv. Cv \<in> snd (translate \<Delta> tys C2) \<Longrightarrow> ConcreteSemantics.wf_abs_stmt (tcfe \<Delta> tys) Cv"
         by (metis Cpar.prems(4) Un_iff snd_eqD translate.simps(9))
       show "well_typed_cmd tys C2"
         using Cpar.prems(2) by auto
-      show "wf_stmt tys \<Gamma> C2"
+      show "wf_stmt \<Delta> tys C2"
         using Cpar.prems(1) by auto
     qed
   qed
@@ -1131,48 +1124,48 @@ next
   show ?case
   proof (rule invariant_translate_if)
     fix P Q
-    show "invariant_translate tys \<Gamma> P C1 Q"
+    show "invariant_translate \<Delta> tys P C1 Q"
     proof (rule Cif(1))
-      show "wf_stmt tys \<Gamma> C1"
+      show "wf_stmt \<Delta> tys C1"
         using Cif.prems(1) by auto
       show "well_typed_cmd tys C1"
         using Cif.prems(2) by auto
-      show "ConcreteSemantics.wf_abs_stmt (tcfe tys) (fst (translate tys \<Gamma> C1))"
+      show "ConcreteSemantics.wf_abs_stmt (tcfe \<Delta> tys) (fst (translate \<Delta> tys C1))"
         using Cif.prems(3) by fastforce
-      show "\<And>Cv. Cv \<in> snd (translate tys \<Gamma> C1) \<Longrightarrow> ConcreteSemantics.wf_abs_stmt (tcfe tys) Cv"
+      show "\<And>Cv. Cv \<in> snd (translate \<Delta> tys C1) \<Longrightarrow> ConcreteSemantics.wf_abs_stmt (tcfe \<Delta> tys) Cv"
         by (metis Cif.prems(4) Un_iff snd_eqD translate.simps(8))
     qed
-    show "invariant_translate tys \<Gamma> P C2 Q"
+    show "invariant_translate \<Delta> tys P C2 Q"
     proof (rule Cif(2))
-      show "wf_stmt tys \<Gamma> C2"
+      show "wf_stmt \<Delta> tys C2"
         using Cif.prems(1) by auto
       show "well_typed_cmd tys C2"
         using Cif.prems(2) by auto
-      show "ConcreteSemantics.wf_abs_stmt (tcfe tys) (fst (translate tys \<Gamma> C2))"
+      show "ConcreteSemantics.wf_abs_stmt (tcfe \<Delta> tys) (fst (translate \<Delta> tys C2))"
         using Cif.prems(3) by fastforce
-      show "\<And>Cv. Cv \<in> snd (translate tys \<Gamma> C2) \<Longrightarrow> ConcreteSemantics.wf_abs_stmt (tcfe tys) Cv"
+      show "\<And>Cv. Cv \<in> snd (translate \<Delta> tys C2) \<Longrightarrow> ConcreteSemantics.wf_abs_stmt (tcfe \<Delta> tys) Cv"
         by (metis Cif.prems(4) Un_iff snd_eqD translate.simps(8))
     qed
   qed
 next
   case (Cwhile b I C)
-  let ?I = "make_semantic_assertion_untyped \<Gamma> (tcfes tys) I"
+  let ?I = "make_semantic_assertion_untyped \<Delta> (tcfes tys) I"
   show ?case
   proof (rule invariant_translate_while)
-    show "ConcreteSemantics.wf_abs_stmt (tcfe tys) (ConcreteSemantics.havoc_list (wrL C))"
+    show "ConcreteSemantics.wf_abs_stmt (tcfe \<Delta> tys) (ConcreteSemantics.havoc_list (wrL C))"
       using Cwhile.prems(3) by simp
-    show "wf_stmt tys \<Gamma> (Cwhile b I C)"
+    show "wf_stmt \<Delta> tys (Cwhile b I C)"
       using Cwhile.prems(1) by auto
-    fix P Q show "invariant_translate tys \<Gamma> P C Q"
+    fix P Q show "invariant_translate \<Delta> tys P C Q"
     proof (rule Cwhile(1)[of P Q])
-      show "wf_stmt tys \<Gamma> C"
+      show "wf_stmt \<Delta> tys C"
         using Cwhile.prems(1) by auto
       show "well_typed_cmd tys C"
         using Cwhile.prems(2) by auto
-      have "ConcreteSemantics.wf_abs_stmt (tcfe tys) (Inhale (?I \<inter> assertify_bexp b);; fst (translate tys \<Gamma> C);; Exhale (inhalify tys ?I))"
+      have "ConcreteSemantics.wf_abs_stmt (tcfe \<Delta> tys) (Inhale (?I \<inter> assertify_bexp b);; fst (translate \<Delta> tys C);; Exhale (inhalify \<Delta> tys ?I))"
         using Cwhile.prems(4) by fastforce
-      then show "ConcreteSemantics.wf_abs_stmt (tcfe tys) (fst (translate tys \<Gamma> C))" by force
-      show "\<And>Cv. Cv \<in> snd (translate tys \<Gamma> C) \<Longrightarrow> ConcreteSemantics.wf_abs_stmt (tcfe tys) Cv"
+      then show "ConcreteSemantics.wf_abs_stmt (tcfe \<Delta> tys) (fst (translate \<Delta> tys C))" by force
+      show "\<And>Cv. Cv \<in> snd (translate \<Delta> tys C) \<Longrightarrow> ConcreteSemantics.wf_abs_stmt (tcfe \<Delta> tys) Cv"
         using Cwhile.prems(4) by auto
     qed
   qed
@@ -1181,66 +1174,59 @@ qed (simp_all add: invariant_translate_skip invariant_translate_free invariant_t
 
 
 lemma atrue_semi_typed:
-  "ConcreteSemantics.semi_typed (tcfe tys) (atrue tys)"
+  "ConcreteSemantics.semi_typed (tcfe \<Delta> tys) (atrue \<Delta> tys)"
   by (metis ConcreteSemantics.semi_typedI atrue_def comp_apply member_filter)
 
 (*
 lemma self_framing_atrue:
-  "self_framing (atrue tys)"
+  "self_framing (atrue \<Delta> tys)"
 proof (rule self_framingI)
 *)
 
 lemma t_entails_inhalify:
-  "t_entails tys P (inhalify tys P)"
+  "t_entails \<Delta> tys P (inhalify \<Delta> tys P)"
   by (simp add: ConcreteSemantics.entails_typed_def TypedEqui.typed_state_then_stabilize_typed)
 
 
 theorem sound_translation:
-  assumes "wf_stmt tys \<Gamma> C"
+  assumes "wf_stmt \<Delta> tys C"
       and "well_typed_cmd tys C"
-      and "ConcreteSemantics.wf_abs_stmt (tcfe tys) (fst (translate tys \<Gamma> C))"
-      and "\<And>Cv. Cv \<in> snd (translate tys \<Gamma> C) \<Longrightarrow> ConcreteSemantics.wf_abs_stmt (tcfe tys) Cv"
+      and "ConcreteSemantics.wf_abs_stmt (tcfe \<Delta> tys) (fst (translate \<Delta> tys C))"
+      and "\<And>Cv. Cv \<in> snd (translate \<Delta> tys C) \<Longrightarrow> ConcreteSemantics.wf_abs_stmt (tcfe \<Delta> tys) Cv"
       and "TypedEqui.wf_assertion P \<and> TypedEqui.wf_assertion Q"
-      and "ConcreteSemantics.verifies_set (tcfe tys) (atrue tys) (Inhale P;; fst (translate tys \<Gamma> C);; Exhale Q)"
-      and "\<And>Cv. Cv \<in> snd (translate tys \<Gamma> C) \<Longrightarrow> ConcreteSemantics.verifies_set (tcfe tys) (atrue tys) Cv"
+      and "ConcreteSemantics.verifies_set (tcfe \<Delta> tys) (atrue \<Delta> tys) (Inhale P;; fst (translate \<Delta> tys C);; Exhale Q)"
+      and "\<And>Cv. Cv \<in> snd (translate \<Delta> tys C) \<Longrightarrow> ConcreteSemantics.verifies_set (tcfe \<Delta> tys) (atrue \<Delta> tys) Cv"
 
-    shows "(tcfe tys) \<turnstile>CSL [P \<otimes> UNIV] C [Q \<otimes> UNIV]"
+    shows "(tcfe \<Delta> tys) \<turnstile>CSL [P \<otimes> UNIV] C [Q \<otimes> UNIV]"
 proof -
-  thm ConcreteSemantics.Viper_implies_SL_proof[OF assms(6) assms(4)]
 
-  obtain B where "ConcreteSemantics.SL_proof (tcfe tys) (atrue tys) (Inhale P;; fst (translate tys \<Gamma> C);; Exhale Q) B"
+  obtain B where "ConcreteSemantics.SL_proof (tcfe \<Delta> tys) (atrue \<Delta> tys) (Inhale P;; fst (translate \<Delta> tys C);; Exhale Q) B"
     by (metis ConcreteSemantics.Viper_implies_SL_proof ConcreteSemantics.wf_abs_stmt.simps(2) ConcreteSemantics.wf_abs_stmt.simps(3) ConcreteSemantics.wf_abs_stmt.simps(7) assms(3) assms(5) assms(6) atrue_def atrue_self_framing_and_typed atrue_semi_typed test_self_framing)
-
-
-  then obtain B' where "ConcreteSemantics.SL_proof (tcfe tys) ((atrue tys) \<otimes> inhalify tys P) (fst (translate tys \<Gamma> C)) B'" "entails B' (B \<otimes> Q)"
+  then obtain B' where "ConcreteSemantics.SL_proof (tcfe \<Delta> tys) ((atrue \<Delta> tys) \<otimes> inhalify \<Delta> tys P) (fst (translate \<Delta> tys C)) B'" "entails B' (B \<otimes> Q)"
     by blast
 
-
-  show "(tcfe tys) \<turnstile>CSL [P \<otimes> UNIV] C [Q \<otimes> UNIV]"
+  show "(tcfe \<Delta> tys) \<turnstile>CSL [P \<otimes> UNIV] C [Q \<otimes> UNIV]"
   proof (rule RuleConsTyped)
-    show "(tcfe tys) \<turnstile>CSL [inhalify tys P \<otimes> (atrue tys) \<otimes> UNIV] C [B' \<otimes> UNIV]"
-    proof (rule invariant_translateE[of _ _ "inhalify tys P \<otimes> (atrue tys)" C])
-      show "ConcreteSemantics.SL_proof (tcfe tys) (inhalify tys P \<otimes> (atrue tys)) (fst (translate tys \<Gamma> C)) B'"
-        by (metis \<open>ConcreteSemantics.SL_proof (tcfe tys) ((atrue tys) \<otimes> inhalify tys P) (fst (translate tys \<Gamma> C)) B'\<close> add_set_commm)
-      show "invariant_translate tys \<Gamma> (inhalify tys P \<otimes> (atrue tys)) C B'"
-
-
+    show "(tcfe \<Delta> tys) \<turnstile>CSL [inhalify \<Delta> tys P \<otimes> (atrue \<Delta> tys) \<otimes> UNIV] C [B' \<otimes> UNIV]"
+    proof (rule invariant_translateE[of _ _ "inhalify \<Delta> tys P \<otimes> (atrue \<Delta> tys)" C])
+      show "ConcreteSemantics.SL_proof (tcfe \<Delta> tys) (inhalify \<Delta> tys P \<otimes> (atrue \<Delta> tys)) (fst (translate \<Delta> tys C)) B'"
+        by (metis \<open>ConcreteSemantics.SL_proof (tcfe \<Delta> tys) ((atrue \<Delta> tys) \<otimes> inhalify \<Delta> tys P) (fst (translate \<Delta> tys C)) B'\<close> add_set_commm)
+      show "invariant_translate \<Delta> tys (inhalify \<Delta> tys P \<otimes> (atrue \<Delta> tys)) C B'"
         by (meson assms(1) assms(2) assms(3) assms(4) invariant_translate_induct)
-      show "proof_obligations_valid tys (snd (translate tys \<Gamma> C))"
+      show "proof_obligations_valid \<Delta> tys (snd (translate \<Delta> tys C))"
         unfolding proof_obligations_valid_def
-      proof clarify
-        fix Cv assume "Cv \<in> snd (translate tys \<Gamma> C)"
-        then show "\<exists>B. ConcreteSemantics.SL_proof (tcfe tys) (atrue tys) Cv B"
-          using ConcreteSemantics.Viper_implies_SL_proof[of "tcfe tys" "atrue tys" Cv] assms(4) assms(7)
-          by (metis atrue_def atrue_self_framing_and_typed atrue_semi_typed test_self_framing)
+        apply clarify
+        using ConcreteSemantics.Viper_implies_SL_proof[of "tcfe \<Delta> tys" "atrue \<Delta> tys"] assms(4) assms(7)
+        by (metis atrue_def atrue_self_framing_and_typed atrue_semi_typed test_self_framing)
       qed
-    qed
-    show "t_entails tys (P \<otimes> UNIV) (inhalify tys P \<otimes> (atrue tys) \<otimes> UNIV)"
-      by (simp add: ConcreteSemantics.entails_typed_refl add_set_asso t_entails_add t_entails_add_atrue t_entails_inhalify)
-    show "t_entails tys (B' \<otimes> UNIV) (Q \<otimes> UNIV)"
-      by (metis (no_types, lifting) \<open>entails B' (B \<otimes> Q)\<close> add_set_mono atrue_twice_equal drop_conjunct_entails dual_order.trans entails_def subset_entails)
+      show "t_entails \<Delta> tys (P \<otimes> UNIV) (inhalify \<Delta> tys P \<otimes> (atrue \<Delta> tys) \<otimes> UNIV)"
+        by (simp add: ConcreteSemantics.entails_typed_refl add_set_asso t_entails_add t_entails_add_atrue t_entails_inhalify)
+      show "t_entails \<Delta> tys (B' \<otimes> UNIV) (Q \<otimes> UNIV)"
+        by (metis (no_types, lifting) \<open>entails B' (B \<otimes> Q)\<close> add_set_mono atrue_twice_equal drop_conjunct_entails dual_order.trans entails_def subset_entails)
   qed
 qed
+
+
 
 
 end
